CCsub_Soundness.v
@@ -8,6 +8,58 @@ Require Import CCsub_Substitution.
 
 Set Nested Proofs Allowed.
 
+(* States *)
+
+Inductive store_frame : Type :=
+  | store v : value v -> store_frame.
+
+Definition store_ctx : Type := list (atom * store_frame).
+Definition stores (S : store_ctx) (x : atom) (v : exp) (v_value : value v) : Prop :=
+    binds x (store v v_value) S.
+
+Inductive scope (e : exp) : Type :=
+  | mk_scope L : (forall x, x `notin` L -> expr (open_ve e x (`cset_fvar` x))) -> scope e.
+
+Inductive eval_frame : Type :=
+  | cont e : scope e -> eval_frame.
+
+Definition eval_ctx : Type := (list eval_frame).
+
+Inductive state : Type :=
+  | mk_state : store_ctx -> eval_ctx -> exp -> state.
+
+Notation "⟨ S | E | e ⟩" := (mk_state S E e) (at level 1).
+
+Inductive state_final : state -> Prop :=
+  | final_state : forall S a,
+      answer a ->
+      state_final ⟨ S | nil | a ⟩.
+
+Inductive store_typing : store_ctx -> env -> Prop :=
+  | typing_store_nil : store_typing nil nil
+  | typing_store_cons : forall x T v v_value S E,
+      store_typing S E ->
+      typing E v T ->
+      x `notin` dom E ->
+      store_typing ([(x, store v v_value)] ++ S) ([(x, bind_typ T)] ++ E).
+
+Inductive eval_typing (E : env) : eval_ctx -> typ -> typ -> Prop :=
+  | typing_eval_nil : forall T U,
+      wf_env E ->
+      sub E T U ->
+      eval_typing E nil T U
+  | typing_eval_cons : forall L k (k_scope : scope k) K T U V,
+      (forall x, x `notin` L ->
+        typing ([(x, bind_typ T)] ++ E) (open_ve k x (`cset_fvar` x)) U) ->
+      eval_typing E K U V ->
+      eval_typing E (cont k k_scope :: K) T V.
+
+Inductive state_typing : state -> typ -> Prop :=
+  | typing_state : forall S K e E T U,
+      store_typing S E ->
+      eval_typing E K T U ->
+      typing E e T ->
+      state_typing ⟨ S | K | e ⟩ U.
 
 (** TODO check where this is used and maybe use "wellformed" tactic **)
 Lemma wf_typ_extract_typ_arrow : forall C E T1 T2,
@@ -21,8 +73,8 @@ Proof with eauto.
 Qed.
 
 (** TODO check where this is used and maybe use "wellformed" tactic **)
-Lemma typing_extract_typ_arrow : forall E Q e C T1 T2,
-  typing E Q e (typ_capt C (typ_arrow T1 T2)) ->
+Lemma typing_extract_typ_arrow : forall E e C T1 T2,
+  typing E e (typ_capt C (typ_arrow T1 T2)) ->
   exists L, forall x, x `notin` L ->
     wf_typ ([(x, bind_typ T1)] ++ E) (dom E `union` singleton x) (dom E) (open_ct T2 (`cset_fvar` x)).
 Proof with eauto.
@@ -33,12 +85,12 @@ Qed.
 (* ********************************************************************** *)
 (** ** Canonical forms (14) *)
 
-Lemma canonical_form_abs : forall Q e U1 U2 C,
+Lemma canonical_form_abs : forall e U1 U2 C,
   value e ->
-  typing empty Q e (typ_capt C (typ_arrow U1 U2)) ->
+  typing empty e (typ_capt C (typ_arrow U1 U2)) ->
   exists V, exists e1, e = exp_abs V e1.
 Proof.
-  intros Q e U1 U2 C Val Typ.
+  intros e U1 U2 C Val Typ.
   remember empty.
   remember (typ_arrow U1 U2).
   revert U1 U2 Heqp Heql.
@@ -51,12 +103,12 @@ Proof.
     eapply IHTyp; eauto.
 Qed.
 
-Lemma canonical_form_tabs : forall Q e U1 U2 C,
+Lemma canonical_form_tabs : forall e U1 U2 C,
   value e ->
-  typing empty Q e (typ_capt C (typ_all U1 U2)) ->
+  typing empty e (typ_capt C (typ_all U1 U2)) ->
   exists V, exists e1, e = exp_tabs V e1.
 Proof.
-  intros Q e U1 U2 C Val Typ.
+  intros e U1 U2 C Val Typ.
   remember empty.
   remember (typ_all U1 U2).
   revert U1 U2 Heqp Heql.
@@ -86,14 +138,17 @@ Proof with eauto.
   - exists C. exists P...
 Qed.
 
-Lemma typing_ctx_free_tvar : forall E Q k T,
-  E @ Q |-ctx k ~: T ->
+(*
+Lemma typing_state_free_tvar : forall S E,
+  store_typing S E ->
   no_type_bindings E.
 Proof with eauto.
   intros. unfold no_type_bindings; intros.
   induction H...
   * intro. binds_cases H...
+  * intro.s 
 Qed.
+*)
 
 Fixpoint env_fv_ct (F : env) {struct F} : atoms :=
   match F with
@@ -102,238 +157,2113 @@ Fixpoint env_fv_ct (F : env) {struct F} : atoms :=
   | (_, bind_sub T) :: F' => (fv_ct T) `u`A (env_fv_ct F')
   end.
 
-Lemma binds_sig_unique : forall T1 T2 l Q,
-    Signatures.binds l (bind_sig T1) Q ->
-    Signatures.binds l (bind_sig T2) Q ->
-    T1 = T2.
-Proof.
-  intros* ? ?.
-  congruence.
+Lemma stores_unique : forall S x v1 v1_value v2 v2_value,
+  stores S x v1 v1_value ->
+  stores S x v2 v2_value ->
+  v1 = v2.
+Proof with eauto*.
+  intros * stores1 stores2.
+  unfold stores, binds in *.
+  rewrite stores1 in stores2.
+  inversion stores2...
 Qed.
 
-Lemma typing_inversion_lvar : forall E Q l T,
-  E @ Q |-t (exp_lvar l) ~: T ->
-  exists C P, T = typ_capt C P.
-Proof.
-  intros * H.
-  dependent induction H; eauto.
-  forwards (C & P & ?): IHtyping l; eauto; subst.
-  inversion select (sub _ (typ_capt C P) _); subst.
-  eauto.
+Lemma wf_cset_notin_fvars : forall x E A C,
+  wf_cset E A C ->
+  x `~in`A dom E ->
+  x `~in`A (`cset_fvars` C).
+Proof with eauto*.
+  intros * WfC NotIn.
+  induction WfC.
+  enough (fvars `c`A dom E) by fsetdec.
+  intros y yIn.
+  destruct (H y ltac:(fsetdec)) as [T [B|B]]; eapply binds_In...
 Qed.
 
-Lemma fv_le_vs_free_for_cv: forall v,
-  fv_le v `c`L `cset_lvars` (free_for_cv v).
-Proof.
-  intros *.
-  dependent induction v; simpl in *; trivial.
-  all: lsetdec.
+Lemma wf_typ_notin_fv_ct : forall x E Ap Am T,
+  wf_typ E Ap Am T ->
+  x `~in`A dom E ->
+  x `~in`A fv_ct T
+with wf_pretyp_notin_fv_cpt : forall x E Ap Am P,
+  wf_pretyp E Ap Am P ->
+  x `~in`A dom E ->
+  x `~in`A fv_cpt P.
+Proof with eauto*.
+{ intros * WfT NotIn.
+  induction WfT; simpl.
+  - fsetdec.
+  - assert (x `~in`A (`cset_fvars` C)) by (applys wf_cset_notin_fvars; eauto*).
+    assert (x `~in`A fv_cpt P) by (applys wf_pretyp_notin_fv_cpt; eauto*).
+    fsetdec.
+}
+{ intros * WfP NotIn.
+  induction WfP; simpl.
+  - fsetdec.
+  - assert (x `~in`A fv_ct T1) by (applys wf_typ_notin_fv_ct; eauto*).
+    pick fresh y and specialize H0.
+    assert (x `~in`A fv_ct T2).
+    { eapply notin_fv_ct_open_ct.
+      eapply wf_typ_notin_fv_ct.
+      apply H0.
+      simpl.
+      assert (x <> y) by (clear - Fr; fsetdec).
+      clear Fr.
+      fsetdec.
+    }
+    clear - H1 H2.
+    fsetdec.
+  - assert (x `~in`A fv_ct T1) by (applys wf_typ_notin_fv_ct; eauto*).
+    pick fresh y and specialize H0.
+    assert (x `~in`A fv_ct T2).
+    { eapply notin_fv_ct_open_tt.
+      eapply wf_typ_notin_fv_ct.
+      apply H0.
+      simpl.
+      assert (x <> y) by (clear - Fr; fsetdec).
+      clear Fr.
+      fsetdec.
+    }
+    clear - H1 H2.
+    fsetdec.
+}
 Qed.
 
-Lemma subcapt_is_label_subset : forall E C D,
-  ~ `* in` D ->
-  E |-sc C <: D ->
-  `cset_lvars` C `c`L `cset_lvars` D.
-Proof with eauto.
-  intros * Notin Hsc.
-  dependent induction Hsc.
-  - congruence.
-  - lsetdec.
-  - lsetdec.
-  - lsetdec.
-  - lsetdec.
-  - lsetdec.
-  - intros l lIn.
-    specialize (H2 l lIn); simpl in H2.
-    clear H0 H1 H3.
-    dependent induction H2; try congruence.
-    + assert (l `in`L {l}L) as HA by lsetdec.
-      rewrite <- x1 in HA.
-      exfalso; lsetdec.
-    + assert (l `in`L {l}L) as HA by lsetdec.
-      rewrite <- x in HA.
-      assert (l0 = l) by lsetdec; subst; clear HA.
-      destruct b0; congruence.
-    + assert (l `in`L {l}L) as HA by lsetdec.
-      rewrite <- x1 in HA.
-      exfalso; lsetdec.
-    + assert (l `in`L {l}L) as HA by lsetdec.
-      rewrite <- x1 in HA.
-      exfalso; lsetdec.
-    + eapply (H3 l)...
-      lsetdec.
+Lemma wf_env_bound_implies_wf_typ : forall E x T,
+  wf_env E ->
+  bound x T E ->
+  wf_typ_in E T.
+Proof with eauto*.
+  intros * WfEnv Bound.
+  induction WfEnv.
+  - Case "wf_env_empty".
+    destruct Bound; inversion H.
+  - Case "wf_env_sub".
+    destruct Bound.
+    + inversion H1; subst.
+      destruct (x == X)...
+      rewrite_env (empty ++ [(X, bind_sub T0)] ++ E).
+      apply wf_typ_in_weakening...
+      apply ok_cons...
+    + inversion H1; subst.
+      destruct (x == X).
+      * inversion H3; subst; clear H3.
+        rewrite_env (empty ++ [(X, bind_sub T)] ++ E).
+        apply wf_typ_in_weakening...
+        apply ok_cons...
+      * rewrite_env (empty ++ [(X, bind_sub T0)] ++ E).
+        apply wf_typ_in_weakening...
+        apply ok_cons... 
+  - Case "wf_env_typ".
+    destruct Bound.
+    + inversion H1; subst.
+      destruct (x == x0); subst.
+      * inversion H3; subst; clear H3.
+        rewrite_env (empty ++ [(x0, bind_typ T)] ++ E).
+        apply wf_typ_weakening with (Ap := dom E) (Am := dom E).
+        -- apply H.
+        -- apply ok_cons...
+        -- repeat rewrite dom_concat.
+           fsetdec.
+        -- repeat rewrite dom_concat.
+           fsetdec.
+      * rewrite_env (empty ++ [(x0, bind_typ T0)] ++ E).
+        apply wf_typ_in_weakening...
+        apply ok_cons...
+    + inversion H1; subst.
+      destruct (x == x0); subst.
+      * inversion H3; subst; clear H3.
+      * rewrite_env (empty ++ [(x0, bind_typ T0)] ++ E).
+        apply wf_typ_in_weakening...
+        apply ok_cons... 
 Qed.
 
-Lemma label_absent_from_cv_is_absent_from_fv : forall l T v E Q,
-  ~ `* in` (cv T) ->
-  ~ l L`in` cv T ->
-  value v ->
-  E @ Q |-t v ~: T ->
-  l `~in`L fv_le v.
-Proof with eauto.
-  intros * NotUniv Notin Val Typ.
-  forwards (U & TypU & SubU): values_have_precise_captures Val Typ.
-  assert (fv_le v `c`L `cset_lvars` (free_for_cv v)) by (apply fv_le_vs_free_for_cv).
-  assert (`cset_lvars` (free_for_cv v) `c`L `cset_lvars` (cv T)). {
-    inversion SubU; subst.
-    eapply subcapt_is_label_subset...
-  }
-  lsetdec.
+Lemma wf_typ_in_notin_fv_ct : forall x E T,
+  wf_typ_in E T ->
+  x `~in`A dom E ->
+  x `~in`A fv_ct T
+with wf_pretyp_in_notin_fv_cpt : forall x E P,
+  wf_pretyp_in E P ->
+  x `~in`A dom E ->
+  x `~in`A fv_cpt P.
+Proof with eauto*.
+{ intros * WfT NotIn.
+  eapply wf_typ_notin_fv_ct with (E := E) (Ap := dom E) (Am := dom E)...
+}
+{ intros * WfP NotIn.
+  eapply wf_pretyp_notin_fv_cpt with (E := E) (Ap := dom E) (Am := dom E)...
+}
 Qed.
 
-Lemma notin_fv_le_open_ee_rec : forall k x C l e,
-  l `~in`L `cset_lvars` C ->
-  l `~in`L fv_le e ->
-  l `~in`L fv_le (open_ee_rec k (exp_fvar x) C e).
-Proof with eauto.
-  intros * NotinC NotinE.
-  generalize dependent k.
-  dependent induction e; intro k; simpl in *...
-  - destruct (k === n); simpl; lsetdec.
-  - lets: IHe1 NotinC __. 1: { lsetdec. }
-    lets: IHe2 NotinC __. 1: { lsetdec. }
-    trivial...
-  - lets: IHe1 NotinC __. 1: { lsetdec. }
-    lets: IHe2 NotinC __. 1: { lsetdec. }
-    trivial...
-Qed.
-
-Lemma notin_fv_le_open_te_rec : forall k T l e,
-  l `~in`L fv_lt T ->
-  l `~in`L fv_le e ->
-  l `~in`L fv_le (open_te_rec k T e).
-Proof with eauto.
-  intros * NotinC NotinE.
-  generalize dependent k.
-  dependent induction e; intro k; simpl in *...
-  - lets: IHe1 NotinC __. 1: { lsetdec. }
-    lets: IHe2 NotinC __. 1: { lsetdec. }
-    trivial...
-  - lets: IHe1 NotinC __. 1: { lsetdec. }
-    lets: IHe2 NotinC __. 1: { lsetdec. }
-    trivial...
-Qed.
-
-Lemma typing_strengthening_sig_absent_label : forall l S E Q v T,
-  E @ [(l, bind_sig S)] ++ Q |-t v ~: T ->
-  l `~in`L fv_le v ->
-  E @ Q |-t v ~: T.
-Proof with eauto.
-  intros* Typ Notin.
+(*
+Lemma typing_of_var_comes_from_binds : forall E (x : atom) T,
+  typing E x T ->
+  exists S, binds x (bind_typ S) E /\ sub E S T.
+Proof with eauto using sub_reflexivity, sub_transitivity.
+  intros * Typ.
+  destruct (typing_regular _ _ _ Typ) as [_ [_ WfT]].
   dependent induction Typ.
-  - constructor...
-    inversion H0...
-  - econstructor...
-    inversion H0...
-  - pick fresh x and apply typing_abs.
-    + trivial.
-    + apply H0.
-      notin_solve.
-    + eapply H2; trivial.
-      * notin_solve.
-      * simpl in Notin.
-        unfold open_ee; eapply notin_fv_le_open_ee_rec...
-  - simpl in Notin.
-    applys typing_app H.
-    + eapply IHTyp1; trivial.
-      lsetdec.
-    + eapply IHTyp2; trivial.
-      lsetdec.
-  - pick fresh X and apply typing_tabs.
-    + trivial.
-    + apply H0.
-      notin_solve.
-    + eapply H2; trivial.
-      * notin_solve.
-      * simpl in Notin.
-        unfold open_te; eapply notin_fv_le_open_te_rec...
-  - simpl in Notin.
-    applys typing_tapp H.
-    eapply IHTyp; trivial.
-    + lsetdec.
-  - applys typing_sub H.
-    eapply IHTyp; trivial.
-  - simpl in Notin.
-    pick fresh x and apply typing_handle.
-    2: { trivial. }
-    eapply H0; trivial.
-    + notin_solve.
-    + unfold open_ee; eapply notin_fv_le_open_ee_rec...
-  - simpl in Notin.
-    eapply typing_do_ret; trivial.
-    + eapply IHTyp1; trivial.
-      lsetdec.
-    + eapply IHTyp2; trivial.
-      lsetdec.
-  - inversion H0; subst.
-    simpl in Notin.
-    eapply typing_lvar...
-    assert (l <> l0) by lsetdec.
-    Signatures.binds_cases H1...
+  - Case "typing_var_tvar".
+    exists X; split...
+  - Case "typing_var".
+    exists (typ_capt C P); split...
+    assert (WfC : wf_cset_in E C).
+    { enough (WfCP : wf_typ_in E (typ_capt C P)) by (inversion WfCP; eauto* ).
+      applys wf_env_binds_typ_implies_wf_typ H H0.
+    }
+    apply sub_capt.
+    + inversion WfC; subst.
+      admit.
+    + eapply sub_pre_reflexivity...
+      inversion WfT...
+      all: clear; fsetdec.
+  - Case "typing_sub".
+    destruct (IHTyp x) as [R [x_binds_R sub_R]]...
+    exists R; split.
+    + apply x_binds_R.
+    + apply sub_transitivity with (Q := S)...
+Admitted.
+*)
+
+(* TODO: move to infrastructure *)
+Lemma notin_open_ve_rec_fv_ve : forall k y z C e,
+  y `notin` (fv_ve e `union` singleton z) ->
+  y `notin` fv_ve (open_ve_rec k z C e).
+Proof with eauto*.
+  intros * y_notin_e_z.
+  generalize dependent k.
+  induction e; intros k; simpl in *;
+  repeat match goal with
+  | v : var |- _ =>
+      destruct v; simpl in *; eauto*;
+      destruct (k === n); eauto*
+  | |- y `notin` (_ `union` _) => apply notin_union
+  | IH : y `notin` _ -> forall k, _ |- _ => apply IH; eauto*
+  end.
 Qed.
 
-Lemma typing_ctx_calculates_bound_capabilities : forall E Q k T,
-  E @ Q |-ctx k ~: T ->
-  Q = bound_capabilities k.
-Proof with eauto.
-  intros * TypCtx.
-  dependent induction TypCtx; simpl; Signatures.simpl_env...
-  - rewrite IHTypCtx.
-    repeat f_equal.
+Lemma notin_open_te_rec_fv_ve : forall k y z e,
+  y `notin` (fv_ve e `union` singleton z) ->
+  y `notin` fv_ve (open_te_rec k z e).
+Proof with eauto*.
+  intros * y_notin_e_z.
+  generalize dependent k.
+  induction e; intros k; simpl in *;
+  repeat match goal with
+  | v : var |- _ =>
+      destruct v; simpl in *; eauto*;
+      destruct (k === n); eauto*
+  | |- y `notin` (_ `union` _) => apply notin_union
+  | IH : y `notin` _ -> forall k, _ |- _ => apply IH; eauto*
+  end.
 Qed.
 
-Lemma notin_fv_ld_is_notin_fv_lt_of_bind_sig : forall l1 l2 Q T,
-  l1 `~in`L fv_ld Q ->
-  Signatures.binds l2 (bind_sig T) Q ->
-  l1 `~in`L fv_lt T.
-Proof with eauto.
-  intros * Notin Bnd.
-  dependent induction Q.
-  - inversion Bnd.
-  - destruct a as (l3 & B).
-    inversion Bnd.
-    destruct (l2 ==== l3).
+Lemma sub_implies_subcapt_cv : forall E S T,
+  sub E S T ->
+  subcapt E (cv S) (cv T).
+Proof with eauto*.
+  intros * Sub.
+  induction Sub; simpl.
+  - apply subcapt_reflexivity with (A := dom E)...
+    constructor.
+    + intros x xIn.
+      assert (x = X) by fsetdec; subst; clear xIn.
+      inversion H0; subst.
+      exists U.
+      apply bound_sub, H2.
     + inversion H0; subst.
-      simpl in Notin.
-      lsetdec.
-    + apply IHQ...
-      simpl in Notin; destruct B.
-      lsetdec.
+      fsetdec.
+  - eapply subcapt_tvar with (T := U)...
+  - assumption.
 Qed.
 
-Lemma extract_nontopness : forall l C R Q E k T,
-  Signatures.binds l (bind_sig (typ_capt C (typ_ret R))) Q ->
-  E @ Q |-ctx k ~: T ->
-  ~ `* in` (cv R).
-Proof with eauto.
-  intros * Bnd TypCtx.
-  dependent induction TypCtx...
-  - inversion Bnd.
-  - destruct (l ==== l0).
-    + assert (Signatures.binds l0 (bind_sig (typ_capt {*} (typ_ret T)))
-                               ([(l0, bind_sig (typ_capt {*} (typ_ret T)))] ++ Q)) as Bnd' by eauto.
-      subst.
-      forwards EQ: binds_sig_unique Bnd Bnd'.
-      inversion EQ; subst; clear EQ...
-    + Signatures.binds_cases Bnd...
+Lemma binds_wf : forall E x T,
+  wf_env E ->
+  binds x (bind_typ T) E ->
+  wf_typ E (dom E `\`A x) (dom E `\`A x) T.
+Proof with eauto*.
+  intros * WfE Binds.
+  induction WfE; simpl.
+  - inversion Binds.
+  - rewrite_env (empty ++ [(X, bind_sub T0)] ++ E).
+    assert (x <> X).
+    { inversion Binds.
+      destruct (x == X)... }
+    replace (({X}A `u`A dom E) `\`A x) with ((dom E `\`A x) `u`A {X}A) by fsetdec.
+    apply wf_typ_weakening with (Ap := dom E `\`A x) (Am := dom E `\`A x).
+    + apply IHWfE.
+      inversion Binds.
+      destruct (x == X)...
+    + apply ok_cons...
+    + fsetdec.
+    + fsetdec.
+  - inversion Binds.
+    destruct (x == x0); subst.
+    + inversion H2; subst.
+      replace (({x0}A `u`A dom E) `\`A x0) with (dom E) by fsetdec.
+      rewrite_env (empty ++ [(x0, bind_typ T)] ++ E).
+      apply wf_typ_weakening with (Ap := dom E) (Am := dom E)...
+      apply ok_cons...
+    + rewrite_env (empty ++ [(x0, bind_typ T0)] ++ E).
+      replace (({x0}A `u`A dom E) `\`A x) with ((dom E `\`A x) `u`A {x0}A) by fsetdec.
+      apply wf_typ_weakening with (Ap := dom E `\`A x) (Am := dom E `\`A x).
+      * apply IHWfE...
+      * apply ok_cons...
+      * fsetdec.
+      * fsetdec.
 Qed.
 
-Lemma wf_sig_weaken_head : forall l S Q,
-  wf_sig ([(l, S)] ++ Q) ->
-  wf_sig Q.
-Proof with eauto.
-  intros.
-  dependent induction H...
+Lemma wf_cset_notin_fvars_atoms : forall E Ap x C,
+  wf_cset E Ap C ->
+  x `~in`A Ap ->
+  x `~in`A (`cset_fvars` C).
+Proof with eauto*.
+  intros * WfC NotIn.
+  inversion WfC; subst...
 Qed.
 
-Lemma preservation : forall e e',
-  typing_state empty e ->
-  step e e' ->
-  typing_state empty e'.
+Lemma wf_typ_notin_cv : forall E Ap Am x T,
+  wf_typ E Ap Am T ->
+  x `~in`A Ap ->
+  x `~in`A (`cset_fvars` (cv T)).
+Proof with eauto*.
+  intros * WfT NotIn.
+  induction WfT; simpl...
+  apply wf_cset_notin_fvars_atoms with (E := E) (Ap := Ap)...
+Qed.
+
+(*
+Lemma subcapt_notin_fvars : forall E C D x,
+  wf_env E ->
+  subcapt E C D ->
+  x `~in`A (`cset_fvars` D) ->
+  `* in` D \/ x `~in`A (`cset_fvars` C).
+Proof with eauto*.
+  intros * WfE Subcapt NotIn.
+  induction Subcapt; subst; simpl in *.
+  - left...
+  - right...
+  - left...
+  - destruct (IHSubcapt WfE NotIn).
+    + left...
+    + right.
+      enough (x <> x0) by fsetdec.
+      intros eq; subst.
+      assert (WfT : wf_typ E (dom E `\`A x0) (dom E `\`A x0) T) by (applys binds_wf WfE H; eauto* ).
+      assert ()
+      
+
+Lemma sub_notin_fv_ct : forall E S T x,
+  sub E S T ->
+  x `~in`A fv_ct T ->
+  x `~in`A fv_ct S
+with sub_pre_notin_fv_ctp : forall E P Q x,
+  sub_pre E P Q ->
+  x `~in`A fv_cpt P ->
+  x `~in`A fv_cpt Q.
+Proof with eauto*.
+{ intros * Sub NotIn.
+  induction Sub; simpl in *.
+  - apply notin_empty.
+  - apply notin_empty.
+  - apply notin_union.
+    +  
+}
+{ intros * Sub NotIn.
+  Guarded.
+
+}
+*)
+
+Lemma typing_strengthening : forall F E x U e T,
+  x `~in`A (fv_cctx F `u`A fv_ct T `u`A fv_ve e) ->
+  typing (F ++ [(x, bind_typ U)] ++ E) e T ->
+  typing (F ++ E) e T.
+Proof with eauto*.
+  intros * NotIn Typ.
+  assert (x `~in`A (dom E `u`A dom F `u`A fv_cctx F `u`A fv_ct T `u`A fv_ve e)).
+  { assert (WfEnv : wf_env (F ++ [(x, bind_typ U)] ++ E)) by applys typing_regular Typ.
+    assert (OkEnv : ok (F ++ [(x, bind_typ U)] ++ E)) by (apply ok_from_wf_env; assumption).
+    enough (x `~in`A (dom E `u`A dom F)) by (clear - H NotIn; fsetdec).
+    clear NotIn Typ WfEnv.
+    dependent induction OkEnv; induction F; inversion x; subst.
+    - fsetdec.
+    - rewrite dom_concat in H.
+      simpl in *.
+      assert (x1 <> x0) by (clear - H; fsetdec).
+      enough (x1 `~in`A (dom E `u`A dom F)) by fsetdec.
+      eapply IHOkEnv...
+  } 
+  clear NotIn; rename H into NotIn.
+  dependent induction Typ; simpl in NotIn.
+  - Case "typing_var_tvar".
+    assert (x <> x0) by (clear - NotIn; fsetdec).
+    apply typing_var_tvar.
+    + apply wf_env_strengthening_typ with (x := x) (T := U)...
+    + apply binds_remove_mid_cons with (y := x) (b := bind_typ U)...
+  - Case "typing_var".
+    assert (x <> x0) by (clear - NotIn; fsetdec).
+    apply typing_var with (C := C).
+    + apply wf_env_strengthening_typ with (x := x) (T := U)...
+    + apply binds_remove_mid_cons with (y := x) (b := bind_typ U)...
+  - Case "typing_abs".
+    pick fresh y and apply typing_abs.
+    + unfold wf_typ_in.
+      apply wf_typ_in_strengthen_typ with (x := x) (U := U).
+      * clear - NotIn; fsetdec.
+      * apply H.
+    + rewrite_env (([(y, bind_typ V)] ++ F) ++ E).
+      replace (dom (F ++ E) `u`A {y}A) with ((dom (F ++ [(x, bind_typ U)] ++ E) `u`A {y}A) `\`A x).
+      replace (dom (F ++ E)) with (dom (F ++ [(x, bind_typ U)] ++ E) `\`A x).
+      eapply wf_typ_strengthen_typ.
+      * rewrite dom_concat; simpl.
+        assert (x <> y) by (clear - Fr; fsetdec).
+        clear - NotIn H3.
+        repeat apply notin_union.
+        -- fsetdec.
+        -- fsetdec.
+        -- fsetdec.
+        -- eapply notin_open_ct_rec_fv_ct...
+      * apply H0.
+        clear - Fr; fsetdec.
+      * repeat rewrite dom_concat.
+        clear - NotIn.
+        notin_simpl; simpl.
+        clear - H H1.
+        fsetdec.
+      * repeat rewrite dom_concat.
+        assert (x <> y) by (clear - Fr; fsetdec).
+        clear - NotIn H3.
+        notin_simpl; simpl.
+        clear - H H3 H1.
+        fsetdec.
+    + rewrite_env (([(y, bind_typ V)] ++ F) ++ E).
+      apply H2 with (x0 := y) (x1 := x) (U0 := U).
+      * clear - Fr; fsetdec.
+      * reflexivity.
+      * repeat rewrite dom_concat.
+        assert (x <> y) by (clear - Fr; fsetdec).
+        clear - NotIn H3.
+        notin_simpl; simpl.
+        repeat apply notin_union.
+        -- apply H.
+        -- apply notin_singleton, H3.
+        -- apply notin_empty.
+        -- apply H1.
+        -- apply H2.
+        -- apply H0.
+        -- apply notin_open_ct_rec_fv_ct.
+           clear - H3 H7; fsetdec.
+        -- apply notin_open_ve_rec_fv_ve.
+           clear - H5 H3; fsetdec.
+  - Case "typing_app".
+    apply typing_app with (T1 := T1) (Cf := Cf).
+    + apply IHTyp1 with (x0 := x) (U0 := U).
+      reflexivity.
+      simpl.
+      assert (WfFE : wf_env (F ++ E)).
+      { apply wf_env_strengthening_typ with (x := x) (T := U)...
+        applys typing_regular Typ1.
+      }
+      assert (exists Cf', subcapt (F ++ E) Cf' Cf /\ x `~in`A (`cset_fvars` Cf')).
+      { eremember (typ_capt Cf (typ_arrow T1 T2)) as TFun.
+        assert (Sub : sub (F ++ E) TFun (typ_capt Cf (typ_arrow T1 T2))).
+        { subst.
+          eapply sub_reflexivity with (Ap := dom (F ++ E)) (Am := dom (F ++ E))...
+          apply wf_typ_in_strengthen_typ with (x := x) (U := U).
+          admit.
+          admit.
+        }
+        clear - NotIn Sub Typ1.
+        generalize dependent Sub.
+        dependent induction Typ1.
+        - intros Sub.
+          exists (`cset_fvar` f).
+          split...
+          eapply subcapt_var with (T := X).
+          + apply binds_remove_mid_cons in H0...
+          + eapply subcapt_tvar.
+            * admit.
+            * admit.  
+        - exists (`cset_fvar` f).
+          split...
+          inversion Sub; subst...
+        - intros Sub.
+          assert (Sub' : sub (F ++ E) S T).
+          { eapply sub_strengthening with (x := x) (U := U).
+            - repeat apply notin_union.
+              + clear - NotIn; fsetdec.
+              + admit.
+              + assert (wf_typ_in (F ++ E) T) by applys sub_regular Sub.
+                apply wf_typ_notin_fv_ct with (E := F ++ E) (Ap := dom (F ++ E)) (Am := dom (F ++ E))...
+            - assumption.
+          }
+          admit. 
+          (* eapply IHTyp1 with (F0 := F) (E0 := E)... *)
+      }
+      assert (WfCf : wf_cset_in (F ++ [(x, bind_typ U)] ++ E) Cf).
+      { enough (WfCapt : wf_typ_in (F ++ [(x, bind_typ U)] ++ E) (typ_capt Cf (typ_arrow T1 T2))) by (inversion WfCapt; eauto* ).
+        applys typing_regular Typ1.
+      }
+      inversion WfCf; subst.
+      clear - NotIn H0.
+      repeat rewrite dom_concat in H0.
+      simpl in H0 |- *.
+      repeat apply notin_union...
+      * notin_simpl.
+        admit.
+      * admit.
+      * eapply notin_fv_ct_open_ct with (C := `cset_fvar` x0)...
+    + apply IHTyp2 with (x1 := x) (U0 := U).
+      reflexivity.
+      clear - NotIn.
+      simpl.
+      repeat apply notin_union...
+      admit.
+  - Case "typing_let".
+    pick fresh y and apply typing_let.
+    + apply IHTyp with (x0 := x) (U0 := U).
+      reflexivity.
+      repeat apply notin_union...
+      admit.  
+    + rewrite_env (([(y, bind_typ T1)] ++ F) ++ E).
+      apply H0 with (x0 := y) (x1 := x) (U0 := U).
+      * clear - Fr; fsetdec.
+      * reflexivity.
+      * repeat rewrite dom_concat.
+        assert (x <> y) by (clear - Fr; fsetdec).
+        clear - NotIn H1.
+        notin_simpl; simpl.
+        repeat apply notin_union.
+        -- apply H.
+        -- apply notin_singleton, H1.
+        -- apply notin_empty.
+        -- apply H2.
+        -- admit.
+        -- apply H0.
+        -- apply H3.
+        -- apply notin_open_ve_rec_fv_ve.
+           clear - H6 H1; fsetdec.
+  - Case "typing_tabs".
+    pick fresh Y and apply typing_tabs.
+    + apply wf_typ_in_strengthen_typ with (x := x) (U := U).
+      * clear - NotIn; fsetdec.
+      * assumption.
+    + rewrite_env (([(Y, bind_sub V)] ++ F) ++ E).
+      replace (dom (F ++ E)) with (dom (F ++ [(x, bind_typ U)] ++ E) `\`A x).
+      eapply wf_typ_strengthen_typ.
+      * rewrite dom_concat; simpl.
+        assert (x <> Y) by (clear - Fr; fsetdec).
+        clear - NotIn H3.
+        repeat apply notin_union.
+        -- fsetdec.
+        -- fsetdec.
+        -- fsetdec.
+        -- eapply notin_open_tt_rec_fv_ct...
+      * apply H0.
+        clear - Fr; fsetdec.
+      * repeat rewrite dom_concat.
+        clear - NotIn.
+        notin_simpl; simpl.
+        clear - H H1.
+        fsetdec.
+    + rewrite_env (([(Y, bind_sub V)] ++ F) ++ E).
+      apply H2 with (X := Y) (x0 := x) (U0 := U).
+      * clear - Fr; fsetdec.
+      * reflexivity.
+      * repeat rewrite dom_concat.
+        assert (x <> Y) by (clear - Fr; fsetdec).
+        clear - NotIn H3.
+        notin_simpl; simpl.
+        repeat apply notin_union.
+        -- apply H.
+        -- apply notin_singleton, H3.
+        -- apply notin_empty.
+        -- apply H1.
+        -- apply H2.
+        -- apply H0.
+        -- apply notin_open_tt_rec_fv_ct.
+           simpl.
+           clear - H3 H7; fsetdec.
+        -- apply notin_open_te_rec_fv_ve.
+           clear - H5 H3; fsetdec.
+  - Case "typing_tapp".
+    apply typing_tapp with (C := C) (T1 := T1).
+    + apply IHTyp with (x1 := x) (U0 := U).
+      reflexivity.
+      assert (WfC : wf_cset_in (F ++ [(x, bind_typ U)] ++ E) C).
+      { enough (WfCapt : wf_typ_in (F ++ [(x, bind_typ U)] ++ E) (typ_capt C (typ_all T1 T2))) by (inversion WfCapt; eauto* ).
+        applys typing_regular Typ.
+      }
+      inversion WfC; subst.
+      clear - NotIn H1.
+      repeat rewrite dom_concat in H1.
+      simpl in H1 |- *.
+      repeat apply notin_union.
+      * fsetdec.
+      * fsetdec.
+      * fsetdec.
+      * admit.
+      * admit.
+      * eapply notin_fv_ct_open_tt with (U := T)...
+      * fsetdec.
+    + apply sub_strengthening with (x := x) (U := U).
+      2: assumption.
+      clear - NotIn.
+      repeat apply notin_union.
+      * fsetdec.
+      * admit.
+      * admit.
+  - Case "typing_sub".
+    apply typing_sub with (S := S).
+    + apply IHTyp with (x0 := x) (U0 := U).
+      reflexivity.
+      repeat apply notin_union.
+      * fsetdec.
+      * fsetdec.
+      * fsetdec.
+      * admit.
+      * fsetdec.
+    + apply sub_strengthening with (x := x) (U := U).
+      2: assumption.
+      repeat apply notin_union.
+      * fsetdec.
+      * admit.
+      * fsetdec.
+Admitted.
+
+Lemma typing_var_inversion : forall E (x : atom) T,
+  typing E x T ->
+     (exists C P, binds x (bind_typ (typ_capt C P)) E /\ sub E (typ_capt (`cset_fvar` x) P) T)
+  \/ (exists X : atom, binds x (bind_typ X) E /\ sub E X T).
+Proof with eauto*.
+  intros * Typ.
+  dependent induction Typ.
+  - Case "typing_var_tvar".
+    right.
+    exists X.
+    split...
+    apply sub_refl_tvar...
+    apply wf_env_bound_implies_wf_typ with (x := x)...
+  - Case "typing_capt".
+    left.
+    exists C, P.
+    split...
+    apply sub_reflexivity with (Ap := dom E) (Am := dom E)...
+    apply wf_typ_capt.
+    + apply wf_concrete_cset.
+      * intros y yIn; assert (y = x) by (clear - yIn; fsetdec); subst...
+      * enough (x `in`A dom E) by fsetdec.
+        eapply binds_In... 
+    + enough (WfCP : wf_typ_in E (typ_capt C P)) by (inversion WfCP; eauto*).
+      apply wf_env_bound_implies_wf_typ with (x := x)...
+  - Case "typing_sub".
+    destruct (IHTyp x eq_refl) as [[C [P [xBinds Sub]]] | [X [xBinds Sub]]].
+    + left.
+      exists C, P.
+      split...
+      apply sub_transitivity with (Q := S)...
+    + right.
+      exists X.
+      split...
+      apply sub_transitivity with (Q := S)...
+Qed.
+
+Lemma sub_capt_inversion : forall E C P T,
+  sub E (typ_capt C P) T ->
+  exists D Q, T = typ_capt D Q
+           /\ subcapt E C D
+           /\ sub_pre E P Q.
+Proof with eauto*.
+  intros * Sub; inversion Sub...
+Qed.
+
+Inductive binds_sub_trans : atom -> cap -> pretyp -> env -> Prop :=
+  | binds_sub_trans_concrete : forall E X C P,
+      binds X (bind_sub (typ_capt C P)) E ->
+      binds_sub_trans X C P E
+  | binds_sub_trans_indirect : forall E (X Y : atom) C P,
+      binds X (bind_sub Y) E ->
+      binds_sub_trans Y C P E ->
+      binds_sub_trans X C P E.
+
+Inductive binds_typ_trans : atom -> cap -> pretyp -> env -> Prop :=
+  | binds_typ_trans_concrete : forall E x C P,
+      binds x (bind_typ (typ_capt C P)) E ->
+      binds_typ_trans x C P E
+  | binds_typ_trans_indirect : forall E (x X : atom) C P,
+      binds x (bind_typ X) E ->
+      binds_sub_trans X C P E ->
+      binds_typ_trans x C P E.
+
+Hint Constructors binds_sub_trans binds_typ_trans : core.
+
+Lemma binds_sub_trans_weakening : forall G F E X C P,
+  ok (G ++ F ++ E) ->
+  binds_sub_trans X C P (G ++ E) ->
+  binds_sub_trans X C P (G ++ F ++ E).
+Proof with eauto*.
+  intros * OkGFE Binds.
+  dependent induction Binds...
+Qed.
+
+(*
+Lemma sub_var_capt_inversion : forall E (X : atom) C P,
+  sub E X (typ_capt C P) ->
+  exists D Q, binds_sub_trans X D Q E
+           /\ subcapt E D C
+           /\ sub_pre E Q P.
+Proof with eauto*.
+  intros * Sub.
+  assert (WfEnv : wf_env E) by applys sub_regular Sub.
+  generalize dependent X.
+  induction WfEnv; intros X0 Sub; inversion Sub; subst.
+  - inversion H0.
+  - destruct (X0 == X); subst.
+    + inversion H2; subst.
+      destruct (X == X); try (contradict n; reflexivity).
+      inversion H3; subst.
+      clear e H3 H2.
+      admit.
+    + 
+*)
+
+(*
+Lemma typing_var_capt_inversion : forall E (x : atom) C P,
+  typing E x (typ_capt C P) ->
+  exists D Q, binds x (bind_typ (typ_capt D Q)) E
+           /\ subcapt E (`cset_fvar` x) C
+           /\ sub_pre E P Q.
+Proof with eauto*.
+  intros * Typ.
+  dependent induction Typ.
+  - exists C0, P.
+    repeat split...
+    + apply subcapt_reflexivity with (A := dom E)...
+      econstructor.
+      * intros z zIn; assert (z = x) by (clear - zIn; fsetdec); subst...
+      * enough (x `in`A dom E) by fsetdec.
+        apply binds_In with (a := bind_typ (typ_capt C0 P))...
+    + apply sub_pre_reflexivity with (Ap := dom E) (Am := dom E)...
+      enough (WfC0P : wf_typ_in E (typ_capt C0 P)) by (inversion WfC0P; eauto* ).
+      apply wf_env_bound_implies_wf_typ with (x := x)...
+  - 
+  eremember (typ_capt C P) as T.
+  assert (Sub : sub E T (typ_capt C P)).
+  { subst; apply sub_reflexivity with (Ap := dom E) (Am := dom E)...
+    applys typing_regular Typ.
+  }
+  clear HeqT.
+  dependent induction Typ.
+  - Case "typing_var_tvar".
+    exists C, P.
+    repeat split...
+    + apply binds_typ_trans_indirect with (X := X)...
+      apply binds_sub_trans_concrete.
+  - exists C0, P.
+    repeat split...
+    + apply subcapt_reflexivity with (A := dom E)...
+      constructor.
+      * intros z zIn; assert (z = x) by (clear - zIn; fsetdec); subst; clear zIn...
+      * enough (x `in`A dom E) by fsetdec; apply binds_In with (a := bind_typ (typ_capt C0 P))...
+    + apply sub_pre_reflexivity with (Ap := dom E) (Am := dom E)...
+      enough (WfC0P : wf_typ_in E (typ_capt C0 P)) by (inversion WfC0P; eauto* ).
+      apply wf_env_bound_implies_wf_typ with (x := x)...
+  - 
+*)
+
+(*
+Lemma typing_var_induction : forall E (x : atom) T,
+  typing E x T ->
+  (exists P, sub E (typ_capt (`cset_fvar` x) P) T).
+Proof with eauto*.
+  intros * Typ.
+  dependent induction Typ.
+  -  
+*)
+
+Ltac impossible_typing Typ :=
+  clear - Typ;
+  repeat match type of Typ with
+  | typing ?E ?e ?T =>
+    let S := fresh "S" in
+    eremember T as S eqn:HeqS;
+    assert (Sub : sub E S T) by (subst; eapply sub_reflexivity; eauto*);
+    clear HeqS;
+    dependent induction Typ;
+      [ inversion Sub
+      | (* cannot name IH in the dependent induction tactic, so we need to match *)
+        match goal with 
+        | H : sub ?E S ?T, IH : forall _ _, e = _ -> _ |- _ =>
+            eapply IH; [ eauto | eapply sub_transitivity with (Q := T); eauto* ]; trivial
+        end ]
+  end.
+
+Lemma subcapt_binds : forall x C P E D,
+  wf_env E ->
+  wf_cset_in E C ->
+  wf_pretyp_in E P ->
+  x `~in`A (`cset_fvars` D) ->
+  subcapt ([(x, bind_typ (typ_capt C P))] ++ E) (`cset_fvar` x) D ->
+  subcapt E C D.
+Proof with eauto*.
+  intros * WfE WfC WfP NotIn Sub.
+  dependent induction Sub.
+  - Case "subcapt_universal".
+    apply subcapt_universal...
+    apply wf_concrete_cset.
+    + intros z zIn.
+      inversion H; subst.
+      destruct (H5 z ltac:(fsetdec)) as [T [B|B]]; binds_cases B...
+    + inversion H; subst.
+      rewrite dom_concat in H6; simpl in H6.
+      fsetdec.
+  - Case "subcapt_in".
+    inversion WfC; subst.
+    admit.
+    (* eapply subcapt_set.
+    assert (x0 = x1) by (apply singleton_set_eq, x); subst; clear x H1.
+    apply subcapt_transitivity with (C2 := `cset_fvar` x1)... *)
+  - Case "subcapt_in_univ".
+    admit.
+  - Case "subcapt_var".
+    admit.
+  - Case "subcapt_set".
+    admit.
+Admitted.
+
+Lemma idk : forall x C P E T, 
+  sub ([(x, bind_typ (typ_capt C P))] ++ E) (typ_capt (`cset_fvar` x) P) T ->
+  sub E (typ_capt C P) T.
+Proof with eauto*.
+  intros * Sub.
+  assert (WfEnv : wf_env ([(x, bind_typ (typ_capt C P))] ++ E)) by applys sub_regular Sub.
+  inversion WfEnv; subst; clear WfEnv.
+  inversion H3; subst; clear H3.
+  rename H2 into WfE.
+  rename H4 into NotIn.
+  rename H7 into WfC.
+  rename H8 into WfP.
+  dependent induction Sub.
+  apply sub_capt.
+  - admit.
+  - admit.
+Admitted.
+
+Lemma sub_tvar_inversion : forall E T (X : atom),
+  sub E T X ->
+  exists Y : atom, T = X \/ binds Y (bind_sub X) E.
+Proof with eauto*.
+  intros * Sub.
+  dependent induction Sub...
+  destruct (IHSub X ltac:(reflexivity)) as [Y [Eq | Binds]]; subst.
+  - exists X0. right. apply H.
+  - exists Y. right. apply Binds.
+  Unshelve.
+  apply X.
+Qed.
+
+Lemma sub_pre_arrow_inversion : forall E T1 T2 P,
+  sub_pre E (typ_arrow T1 T2) P ->
+  P = typ_top
+  \/ (exists S1 S2 L, P = typ_arrow S1 S2
+     /\ sub E S1 T1
+     /\ (forall x, x `~in`A L ->
+           sub ([(x, bind_typ S1)] ++ E)
+               (open_ct T2 (`cset_fvar` x))
+               (open_ct S2 (`cset_fvar` x)))).
+Proof with eauto*.
+  intros * Sub.
+  dependent induction Sub...
+  right.
+  exists T0, T3, L.
+  repeat split...
+Qed.
+
+Lemma sub_capt_arrow_inversion : forall E C T1 T2 T,
+  sub E (typ_capt C (typ_arrow T1 T2)) T ->
+  exists D, T = typ_capt D typ_top
+  \/ (exists S1 S2 L, T = typ_capt D (typ_arrow S1 S2)
+     /\ subcapt E C D
+     /\ sub E S1 T1
+     /\ (forall x, x `~in`A L ->
+          sub ([(x, bind_typ S1)] ++ E)
+              (open_ct T2 (`cset_fvar` x))
+              (open_ct S2 (`cset_fvar` x)))).
+Proof with eauto*.
+  intros * Sub.
+  dependent induction Sub.
+  destruct (sub_pre_arrow_inversion _ _ _ _ H0) as [Eq | [S1 [S2 [L [Eq [S1SubT1 T2SubS2]]]]]]; subst.
+  - exists C2...
+  - exists C2.
+    right.
+    exists S1, S2.
+    repeat split...
+Qed.
+
+Lemma typing_abs_implies_sub_arrow : forall E U e T,
+  typing E (exp_abs U e) T ->
+  exists T1 T2, typing E (exp_abs U e) (typ_capt (free_for_cv e) (typ_arrow T1 T2))
+             /\ sub E (typ_capt (free_for_cv e) (typ_arrow T1 T2)) T.
+Proof with eauto*.
+  intros * Typ.
+  assert (WfEnv : wf_env E) by applys typing_regular Typ.
+  assert (WfCV : wf_cset_in E (free_for_cv (exp_abs U e))).
+  { eapply typing_cv... }
+  simpl in WfCV.
+  dependent induction Typ.
+  - exists U, T1.
+    split...
+    apply sub_reflexivity with (Ap := dom E) (Am := dom E)...
+  - destruct (IHTyp U e ltac:(reflexivity) WfEnv WfCV) as [T1 [T2 Sub]].
+    exists T1, T2.
+    split...
+    apply sub_transitivity with (Q := S)...
+Qed.
+
+Lemma typing_abs_all_impossible : forall E U e C T1 T2,
+  ~ typing E (exp_abs U e) (typ_capt C (typ_all T1 T2)).
+Proof with eauto*.
+  intros * Typ.
+  dependent induction Typ.
+
+Lemma typing_val_inversion_aux : forall E v T,
+  value v ->
+  typing E v T ->
+  exists C P, T = typ_capt C P
+  /\ (P = typ_top
+   \/ (exists T1 T2, P = typ_arrow T1 T2)
+   \/ (exists T1 T2, P = typ_all T1 T2)).
+Proof with eauto*.
+  intros * Val Typ.
+  assert (WfEnv : wf_env E) by applys typing_regular Typ.
+  assert (WfCV : wf_cset_in E (free_for_cv v)) by applys typing_cv Typ.
+  inversion Val; subst.
+  - dependent induction Typ...
+    + exists (free_for_cv e1), (typ_arrow T0 T1).
+      repeat split...
+    + destruct (IHTyp T0 e1 ltac:(reflexivity) Val WfEnv WfCV H0) as [C [P [EqS [EqP | [[T2 [T3 EqP]] | [T2 [T3 EqP]]]]]]]; subst.
+      * inversion H; subst.
+        inversion H6; subst.
+        exists C2, typ_top...
+      * inversion H; subst.
+        inversion H6; subst.
+        -- exists C2, typ_top...
+        -- exists C2, (typ_arrow T1 T4)...
+      * inversion Typ; subst.
+        inversion H6; subst.
+        -- exists  
+  - dependent induction Typ...
+    exists (free_for_cv e1), (typ_all T0 T1)...
+*)
+Lemma typing_val_inversion : forall E v T,
+  value v ->
+  typing E v T ->
+  exists C P, typing E v (typ_capt C P)
+  /\ sub E T (typ_capt C P)
+  /\ ((exists T1 T2, P = typ_arrow T1 T2)
+   \/ (exists T1 T2, P = typ_all T1 T2)).
+Proof with eauto*.
+  intros * Val Typ.
+  assert (WfEnv : wf_env E) by applys typing_regular Typ.
+  assert (WfCV : wf_cset_in E (free_for_cv v)) by applys typing_cv Typ.
+  inversion Val; subst.
+  - dependent induction Typ...
+    + exists (free_for_cv e1), (typ_arrow T0 T1).
+      repeat split...
+      apply sub_reflexivity with (Ap := dom E) (Am := dom E)...
+    + destruct (IHTyp T0 e1 ltac:(reflexivity) Val WfEnv WfCV H0) as [C [P [Typ' [Sub' [[T2 [T3 Eq]] | [T2 [T3 Eq]]]]]]]; subst.
+      * repeat eexists.
+  - dependent induction Typ...
+    exists (free_for_cv e1), (typ_all T0 T1)...
+Qed.
+
+Lemma stores_preserves_typing : forall S E x v v_value C P,
+  store_typing S E ->
+  stores S x v v_value ->
+  typing E x (typ_capt C P) ->
+  exists D, typing E v (typ_capt D P).
+Proof with eauto*.
+  intros * StoreTyp xStores Typ.
+  induction StoreTyp; inversion xStores.
+  destruct (x == x0); subst.
+  - Case "x = x0".
+    inversion H2; subst; clear H2.
+    destruct (typing_val_inversion _ _ _ v_value H) as [C' [P' [Typ' [[T1 [T2 Eq]] | [T1 [T2 Eq]]]]]].
+    + SCase "value_abs".
+      exists C'.
+      rewrite_env (empty ++ [(x0, bind_typ T)] ++ E).
+      apply typing_weakening with (F := [(x0, bind_typ T)]).
+    
+    inversion v_value; subst.
+    + destruct (typing_abs_implies_sub_arrow _ _ _ _ H) as [T1 [T2 [Typ' Sub']]].
+      exists (free_for_cv e1).
+      destruct (sub_capt_arrow_inversion _ _ _ _ _ Sub') as [D [Eq | [S1 [S2 [L [Eq [Subcapt [S1SubT1 T2SubS2]]]]]]]].
+      * inversion Eq; subst; clear H2.
+        split.
+        -- apply typing_abs. 
+  - Case "x <> x0".
+
+
+      inversion H2; subst.
+      destruct (typing_var_inversion _ _ _ Typ) as [[C' [P' [x0Binds Sub]]] | [X [x0Binds Sub]]].
+      * inversion x0Binds.
+        destruct (x0 == x0); try (contradict n; reflexivity).
+        inversion H3; subst.
+        clear e H2 H3 IHStoreTyp.
+        exists C'.
+        rewrite_env (empty ++ [(x0, bind_typ (typ_capt C' P'))] ++ E).
+        inversion Sub; subst.
+        assert (WfC'P' : wf_typ_in E (typ_capt C' P')).
+        { applys typing_regular H. }
+        apply typing_sub with (S := typ_capt C' P').
+        -- apply typing_weakening...
+        -- apply sub_capt... 
+           apply subcapt_reflexivity with (A := dom E).
+           apply wf_cset_weakening with (A := dom E)...
+           inversion WfC'P'...
+           simpl.
+           fsetdec.
+        (*
+        apply typing_sub with (S := U).
+        apply H.
+        rewrite_env (empty ++ [(x0, bind_typ U)] ++ E) in UsubT.
+        apply sub_strengthening in UsubT.
+        apply UsubT.
+        simpl.
+        repeat apply notin_union.
+        -- fsetdec.
+        -- destruct (sub_regular _ _ _ UsubT) as [WfEnv _].
+          inversion WfEnv; subst. 
+          eapply wf_typ_in_notin_fv_ct...
+        -- admit.
+        *)
+      * exists C.
+        inversion x0Binds; subst.
+        destruct (x0 == x0); subst...
+        clear e.
+        inversion H3; subst; clear H3.
+        apply typing_sub with (S := X)...
+        rewrite_env (empty ++ [(x0, bind_typ X)] ++ E).
+        apply typing_weakening with (F := [(x0, bind_typ X)])...
+    + Case "x <> y".
+      assert (IHStore : stores S x v v_value).
+      { inversion xStores.
+        destruct (x == x0); try (contradict e; apply n).
+        apply H3.
+      }
+      destruct (IHStoreTyp IHStore) as [D Typ'].
+      * rewrite_env (empty ++ E).
+        apply typing_strengthening with (x := x0) (U := T).
+        -- simpl.
+           repeat apply notin_union...
+           Check capture_prediction.
+        -- assumption.
+      * exists D.
+        apply  
+      assert (IHtyp : typing E x T).
+      { rewrite_env (empty ++ [(x0, bind_typ T0)] ++ E) in Typ.
+        apply typing_strengthening in Typ; simpl.
+        - apply Typ.
+        - repeat apply notin_union.
+          + clear; fsetdec.
+          + admit.
+          + clear - n; fsetdec.   
+      }
+      rewrite_env (empty ++ [(x0, bind_typ T0)] ++ E).
+      apply typing_weakening...
+      apply wf_env_typ.
+      * applys typing_regular H.
+      * applys typing_regular H.
+      * clear - H0; fsetdec.
+Admitted.
+
+Lemma eval_typing_regular : forall E K T U,
+  eval_typing E K T U ->
+  wf_env E /\ wf_typ_in E T /\ wf_typ_in E U.
+Proof with eauto*.
+  intros * EvalTyp.
+  induction EvalTyp; repeat split...
+  pick fresh x and specialize H.
+  destruct (typing_regular _ _ _ H) as [wf_xTE _].
+  inversion wf_xTE; subst...
+Qed.
+
+(*
+Lemma eval_typing_contravariant : forall E K S T U,
+  sub Γ S T ->
+  eval_typing E K T U ->
+  eval_typing E K S U.
+Proof with eauto*.
+  intros *.
+  intros subT eval_typ.
+  generalize dependent T'.
+  induction eval_typ; intros T' subT.
+  - apply typing_eval_nil...
+    apply sub_transitivity with (Q := T)...
+  - eapply typing_eval_cons with (L := L) (U := U)...
+    intros x x_fresh.
+    rewrite_env (empty ++ [(x, bind_typ T')] ++ Γ).
+    eapply typing_specializing...
+Qed.
+*)
+
+Lemma eval_typing_weakening : forall E F G E' T U,
+  eval_typing (G ++ E) E' T U ->
+  wf_env (G ++ F ++ E) ->
+  eval_typing (G ++ F ++ E) E' T U.
+Proof with eauto*.
+  intros * Typ WfEnv.
+  induction Typ.
+  - Case "typing_eval_nil".
+    apply typing_eval_nil...
+    apply sub_weakening...
+  - Case "typing_eval_cons".
+    apply typing_eval_cons with (L := L `union` dom (G ++ F ++ E)) (U := U).
+    + intros x x_fresh.
+      assert (k_typing : typing (([(x, bind_typ T)] ++ G) ++ E) (open_ve k x (`cset_fvar` x)) U) by (apply (H x); eauto).
+      eapply typing_weakening with (F := F) in k_typing.
+      * SSCase "typing".
+        apply k_typing.
+      * SSCase "well formedness".
+        simpl_env.
+        apply wf_env_typ...
+        assert (wf_env_xTGE : wf_env (([(x, bind_typ T)] ++ G) ++ E)).
+        { eapply typing_regular, k_typing. }
+        assert (wf_typ_xTGE_T : wf_typ_in (([(x, bind_typ T)] ++ G) ++ E) T).
+        { apply (wf_typ_from_wf_env_typ x) in wf_env_xTGE.
+          simpl_env.
+          replace ((fix app (l m : env) {struct l} : env :=
+                      match l with
+                      | nil => m
+                      | a :: l1 => a :: app l1 m
+                      end) G E) with (G ++ E) in wf_env_xTGE by reflexivity.
+          rewrite_env (empty ++ [(x, bind_typ T)] ++ G ++ E).
+          apply wf_typ_in_weakening...
+          apply ok_cons...
+          apply ok_from_wf_env.
+          apply wf_env_strengthening with (F := [(x, bind_typ T)]).
+          applys typing_regular k_typing.
+        }
+        simpl_env in *.
+        apply wf_typ_in_weakening with (F := F).
+        -- apply (wf_typ_from_wf_env_typ x)...
+        -- apply ok_from_wf_env...
+    + assumption.
+Qed.
+
+Lemma wf_capt_from_typing_var : forall E x C P,
+  wf_env E ->
+  binds x (bind_typ (typ_capt C P)) E ->
+  wf_cset_in E C /\ wf_pretyp_in E P.
+Proof with eauto*.
+  intros * WfEnv xBinds.
+  induction WfEnv.
+  - Case "wf_env_empty".
+    inversion xBinds.
+  - Case "wf_env_sub".
+    rewrite_env (empty ++ [(X, bind_sub T)] ++ E).
+    assert (binds x (bind_typ (typ_capt C P)) E).
+    { inversion xBinds.
+      destruct_if in H2...
+    }
+    destruct (IHWfEnv H1) as [WfC WfP].
+    split.
+    + apply wf_cset_in_weakening...
+      apply ok_cons...
+    + apply wf_pretyp_in_weakening...
+      apply ok_cons...
+  - Case "wf_env_typ".
+    destruct (x == x0); subst.
+    + SCase "x = x0".
+      inversion xBinds.
+      destruct (x0 == x0); try (contradict n; reflexivity).
+      inversion H2; subst.
+      rewrite_env (empty ++ [(x0, bind_typ (typ_capt C P))] ++ E).
+      split.
+      * apply wf_cset_in_weakening.
+        inversion H; subst...
+        apply ok_cons...
+      * apply wf_pretyp_in_weakening...
+        apply ok_cons...
+    + SCase "x <> x0".
+      rewrite_env (empty ++ [(x0, bind_typ T)] ++ E).
+      assert (binds x (bind_typ (typ_capt C P)) E).
+      { inversion xBinds.
+        destruct_if in H2...
+      }
+      destruct (IHWfEnv H1) as [WfC WfP].
+      split.
+      * apply wf_cset_in_weakening...
+        apply ok_cons...
+      * apply wf_pretyp_in_weakening...
+        apply ok_cons...
+Qed.
+
+Lemma typing_abs_typ_arrow_implies_sub_param : forall E U e C T1 T2,
+  typing E (exp_abs U e) (typ_capt C (typ_arrow T1 T2)) ->
+  sub E T1 U.
+Proof with eauto*.
+  intros * Typ.
+  destruct (typing_regular _ _ _ Typ) as [WfE [_ WfT]].
+  inversion WfT; subst.
+  eremember (exp_abs U e) as abs.
+  eremember (typ_capt C (typ_arrow T1 T2)) as S.
+  rename WfT into WfS.
+  assert (Sub : sub E S (typ_capt C (typ_arrow T1 T2))).
+  { subst.
+    eapply sub_reflexivity with (Ap := dom E) (Am := dom E)...
+  }
+  clear HeqS.
+  induction Typ; inversion Heqabs; subst.
+  - inversion Sub; subst...
+    inversion H11...
+  - eapply IHTyp...
+    apply sub_transitivity with (Q := T)...
+Qed.
+
+Lemma binds_sub_arrow_implies_store_abs : forall S E C TFun T1 T2 f,
+  store_typing S E ->
+  binds f (bind_typ TFun) E ->
+  sub E TFun (typ_capt C (typ_arrow T1 T2)) ->
+  exists U e (abs_value : value (exp_abs U e)), stores S f (exp_abs U e) abs_value /\ sub E T1 U.
+Proof with eauto*.
+  intros * StoreTyp fBinds Sub.
+  eremember (typ_arrow T1 T2) as TFun' eqn:EQ.
+  induction StoreTyp; inversion fBinds; inversion EQ; subst.
+  destruct (f == x).
+  - inversion H2; subst...
+    unfold stores.
+    unfold binds.
+    simpl.
+    destruct (x == x); [ clear e | contradict n; reflexivity ].
+    inversion v_value; subst.
+    + inversion H; subst.
+      * exists T, e1, v_value.
+        inversion Sub; subst.
+        split...
+        inversion H13; subst...
+      * exists T, e1, v_value.
+        split...
+        rewrite_env (empty ++ [(x, bind_typ TFun)] ++ E).
+        apply sub_weakening.
+        -- assert (Typ : typing E (exp_abs T e1) (typ_capt C (typ_arrow T1 T2))).
+           { apply typing_sub with (S := TFun)...
+             rewrite_env (empty ++ [(x, bind_typ TFun)] ++ E) in Sub.
+             apply sub_strengthening in Sub.
+             - assumption.
+             - simpl.
+               repeat apply notin_union.
+               + clear; fsetdec.
+               + inversion Sub; subst.
+                 * clear; fsetdec.
+                 * destruct (sub_regular _ _ _ H5) as [_ [_ WfTyp]].
+                   eapply wf_typ_in_notin_fv_ct...
+               + eapply wf_cset_notin_fvars with (E := E) (A := dom E).
+                 * admit. 
+                 * apply H0.
+               + apply wf_typ_in_notin_fv_ct with (E := E).
+                 * admit.
+                 * apply H0.
+               + apply wf_typ_in_notin_fv_ct with (E := E).
+                 * admit.
+                 * apply H0.
+           }
+           applys typing_abs_typ_arrow_implies_sub_param Typ.
+        -- apply wf_env_typ...
+    + assert (tabs_has_type_T1_arr_T2 : typing E (exp_tabs T e1) (typ_capt C (typ_arrow T1 T2))).
+      { apply typing_sub with (S := TFun)...
+        rewrite_env (empty ++ [(x, bind_typ TFun)] ++ E) in Sub.
+        apply sub_strengthening in Sub.
+        - apply Sub.
+        - destruct (sub_regular _ _ _ Sub) as [WfEnv [WfTFun WfS]].
+          inversion WfEnv; inversion WfS. inversion H16; subst.
+          repeat apply notin_union.
+          + fsetdec.
+          + eapply wf_typ_in_notin_fv_ct...
+          + admit.
+          + admit.
+          + admit. 
+      }
+      admit.
+      (* exfalso; impossible_typing tabs_has_type_T1_arr_T2. *)
+  - assert (Sub' : sub E TFun (typ_capt C (typ_arrow T1 T2))).
+    { rewrite_env (empty ++ [(x, bind_typ T)] ++ E) in Sub.
+      apply sub_strengthening in Sub.
+      - apply Sub.
+      - repeat apply notin_union.
+        + fsetdec.
+        + admit.
+        + admit.
+        + admit.
+        + admit.     
+    }
+    destruct IHStoreTyp as [U [e [abs_value [xv_S_stores_f T1_sub_U]]]]...
+    exists U, e, abs_value.
+    split.
+    + rewrite_env ([(x, store v v_value)] ++ S).
+      apply binds_tail.
+      * trivial.
+      * simpl; fsetdec.
+    + rewrite_env (empty ++ [(x, bind_typ T)] ++ E).
+      apply sub_weakening...
+Admitted.
+
+(*
+Lemma subcapt_open_cset : forall E k C D c,
+  wf_cset_in E c ->
+  subcapt E C D ->
+  subcapt E (open_cset k C c) (open_cset k D c).
+Proof with eauto*.
+  intros * Wfc Subcapt.
+  unfold open_cset.
+  destruct (subcapt_regular _ _ _ Subcapt) as [WfC WfD].
+  inversion WfC; subst; rename H into HC, fvars into fvarsC.
+  inversion WfD; subst; rename H into HD, fvars into fvarsD.
+  destruct_set_mem k c.
+    induction Subcapt.
+    + csetsimpl.
+      Print open_cset.
+      replace (`cset_bvars` c `\`N k) with (`cset_bvars` c).
+      apply subcapt_universal.
+      * inversion H2; subst.
+  - eapply subcapt_reflexivity with (A := dom E)...
+
+Lemma sub_open_ct : forall E T C D,
+  wf_env E ->
+  wf_typ_in E T ->
+  subcapt E C D ->
+  sub E (open_ct T C) (open_ct T D)
+with sub_pre_open_cpt : forall E P C D,
+  wf_env E ->
+  wf_pretyp_in E P ->
+  subcapt E C D ->
+  sub_pre E (open_cpt P C) (open_cpt P D).
+Proof with eauto*.
+{ intros * WfEnv WfTyp Subcapt.
+  induction WfTyp; unfold open_ct; simpl.
+  - apply sub_refl_tvar...
+    apply wf_typ_var with (U := U)...
+    applys binds_In X...
+  - apply sub_capt.
+     
+}
+{ intros * Sub.
+}
+*)
+
+Lemma typing_inv_abs : forall E S1 e1 T,
+  typing E (exp_abs S1 e1) T ->
+  forall U1 U2 C, sub E T (typ_capt C (typ_arrow U1 U2)) ->
+    sub E U1 S1
+  /\ exists S2, exists L, forall x, x `notin` L ->
+    typing ([(x, bind_typ S1)] ++ E) (open_ve e1 x (`cset_fvar` x)) (open_ct S2 (`cset_fvar` x)) /\
+    wf_typ ([(x, bind_typ S1)] ++ E) (dom E `union` singleton x) (dom E) (open_ct U2 (`cset_fvar` x)) /\
+  sub ([(x, bind_typ U1)] ++ E) (open_ct S2 (`cset_fvar` x)) (open_ct U2 (`cset_fvar` x)).
+Proof with auto.
+  intros * Htyp.
+  dependent induction Htyp; intros U1 U2 C Hsub.
+  - Case "typing_abs".
+    inversion Hsub; subst.
+    inversion select (sub_pre _ _ _); subst.
+    split...
+    exists T1.
+    exists (L `union` L0).
+    intros y ?.
+    repeat split.
+    + apply H1...
+    + rewrite_nil_concat.
+      eapply wf_typ_ignores_typ_bindings.
+      apply H13...
+    + trivial...
+  - Case "typing_sub".
+    eauto using (sub_transitivity T).
+Qed.
+
+(*
+Lemma typing_narrowing_typ : forall F z U V E e T,
+  sub E U V ->
+  typing (F ++ [(z, bind_typ V)] ++ E) e T ->
+  typing (F ++ [(z, bind_typ U)] ++ E) e T.
+Proof with simpl_env; eauto using wf_typ_narrowing_typ, wf_env_narrowing_typ.
+  intros * Sub Typ.
+  eremember (F ++ [(z, bind_typ V)] ++ E) as G.
+  generalize dependent F.
+  induction Typ; intros F EQ; subst.
+  - Case "typing_var_tvar".
+    binds_cases H0.
+    + apply typing_var_tvar.
+      * eauto using wf_env_narrowing_typ.
+      * apply binds_weaken_at_head.
+        apply binds_weaken_at_head.
+        eauto.
+        apply ok_from_wf_env, wf_env_strengthening with (F := F)...
+        apply ok_from_wf_env...
+    + inversion H1; subst.
+      apply typing_sub with (S := U)...
+      * rewrite_env (empty ++ (F ++ [(x, bind_typ U)]) ++ E).
+        assert (WfU : wf_typ_in E U) by applys sub_regular Sub.
+        inversion WfU; subst.
+        -- apply typing_var_tvar...
+        -- apply typing_sub with (S := typ_capt (`cset_fvar` x) P).
+           ++ apply typing_var with (C := C)...
+           ++ apply sub_capt...
+              ** eapply subcapt_var with (T := typ_capt C P)...
+                 simpl.
+                 rewrite_env (empty ++ (F ++ [(x, bind_typ (typ_capt C P))]) ++ E).
+                 eapply subcapt_reflexivity with (A := dom (empty ++ (F ++ [(x, bind_typ (typ_capt C P))]) ++ E)).
+                 eapply wf_cset_in_weakening...
+                 repeat rewrite dom_concat...
+                 clear; fsetdec.
+              ** rewrite_env (empty ++ (F ++ [(x, bind_typ (typ_capt C P))]) ++ E).
+                 eapply sub_pre_reflexivity with (Ap := dom E) (Am := dom E)...
+                 rewrite_env (empty ++ (F ++ [(x, bind_typ (typ_capt C P))]) ++ E).
+                 eapply wf_pretyp_weakening with (Ap := dom E) (Am := dom E)...
+                 all: clear; fsetdec.
+      * rewrite_env (empty ++ (F ++ [(x, bind_typ U)]) ++ E).
+        apply sub_weakening...
+    + apply typing_var_tvar...
+  - Case "typing_var".
+    binds_cases H0.
+    + apply typing_var with (C := C).
+      * eauto using wf_env_narrowing_typ.
+      * simpl in Fr0.
+        assert (x <> z) by (clear - Fr0; fsetdec); clear Fr0.
+        apply binds_tail... 
+    + inversion H1; subst; clear H1.
+      inversion Sub; subst.
+      * apply typing_sub with (S := X).
+        -- apply typing_var_tvar...
+        -- eapply sub_trans_tvar with (U := U0).
+           ++ apply binds_tail.
+              apply binds_tail.
+              apply H0.
+              simpl.
+              ** enough (X <> x) by fsetdec.
+                 intros eq; subst.
+                 assert (ok ([(x, bind_typ (typ_capt C P))] ++ E)).
+                 { apply wf_env_strengthening in H.
+                   apply ok_from_wf_env, H.
+                 }
+                 inversion H2; subst.
+                 assert (x `in`A dom E) by applys binds_In H0.
+                 apply (H7 H3).
+              ** assert (ok (F ++ E)).
+                 { assert (ok (F ++ [(x, bind_typ (typ_capt C P))] ++ E)) by applys ok_from_wf_env H.
+                   eapply ok_remove_mid, H2.
+                 }
+                 assert (X `in`A dom E) by applys binds_In H0.
+                 eapply tail_not_in_head with (E := E)...
+           ++ admit.
+      * apply typing_sub with (S := typ_capt (`cset_fvar` x) P1).
+        -- apply typing_var with (C := C1)...
+        -- apply sub_capt.
+           ++ apply subcapt_reflexivity with (A := dom (F ++ [(x, bind_typ (typ_capt C1 P1))] ++ E)).
+              ** apply wf_concrete_cset...
+                 --- intros z zIn.
+                     assert (z = x) by (clear - zIn; fsetdec); subst; clear zIn.
+                     exists (typ_capt C1 P1).
+                     apply bound_typ...
+                 --- clear; fsetdec.
+              ** clear; fsetdec.
+           ++ rewrite_env (empty ++ (F ++ [(x, bind_typ (typ_capt C1 P1))]) ++ E).
+              apply sub_pre_weakening...
+    + assert (WfU : wf_typ_in E U) by applys sub_regular Sub.
+      inversion WfU; subst.
+      * apply typing_sub with (S := typ_capt (`cset_fvar` x) P).
+        -- apply typing_var with (C := C)...
+        -- apply sub_capt...
+           ++ eapply subcapt_var with (T := typ_capt C P)...
+              simpl; simpl_env.
+              admit.
+           ++ rewrite_env (empty ++ (F ++ [(z, bind_typ X)]) ++ E).
+              eapply sub_pre_reflexivity with (Ap := dom (F ++ [(z, bind_typ X)] ++ E)) (Am := dom (F ++ [(z, bind_typ X)] ++ E))...
+              rewrite_env (F ++ empty) in H2.
+              apply binds_weaken with (F := [(z, bind_typ X)] ++ E) in H2.
+              simpl_env in H2.
+              eapply wf_env_narrowing_typ with (U := X) in H...
+              destruct (wf_capt_from_typing_var _ _ _ _ H H2).
+              unfold wf_pretyp_in in H4.
+              replace (dom F `u`A {z}A `u`A dom E) with (dom (F ++ [(z, bind_typ X)] ++ E)).
+              apply H4.
+              repeat rewrite dom_concat; simpl; clear; fsetdec.
+              apply ok_from_wf_env...
+              all: clear; fsetdec.
+      * apply typing_sub with (S := typ_capt (`cset_fvar` x) P0).
+        -- apply typing_var with (C := C0)...
+           apply binds_tail.
+           apply binds_head.
+           apply binds_singleton.
+  - Case "typing_abs".
+    pick fresh x and apply typing_abs.
+    rewrite_env (([(x, bind_typ V)] ++ F) ++ [(z, bind_typ P)] ++ E).
+    apply H0...
+  - Case "typing_tabs".
+    pick fresh X and apply typing_tabs.
+    rewrite_env (([(X, bind_sub V)] ++ F) ++ [(z, bind_typ P)] ++ E).
+    apply H0...
+  - Case "typing_tapp".
+    apply typing_tapp with (T1 := T1).
+    apply IHe_T...
+    apply sub_specializing with (Q := Q)...
+  - Case "typing_let".
+    pick fresh x and apply typing_let...
+    rewrite_env (([(x, bind_typ T1)] ++ F) ++ [(z, bind_typ P)] ++ E).
+    apply H0...
+  - Case "typing_sub".
+    apply typing_sub with (S := S)...
+    apply sub_specializing with (Q := Q)...
+Qed.
+*)
+
+(*
+Lemma eval_typing_sub : forall E K S T U,
+  sub E S T ->
+  eval_typing E K T U ->
+  eval_typing E K S U.
+Proof with eauto*.
+  intros *.
+  intros Sub EvalTyp.
+  generalize dependent S.
+  induction EvalTyp; intros S Sub.
+  - apply typing_eval_nil...
+    apply sub_transitivity with (Q := T)...
+  - eapply typing_eval_cons with (L := L) (U := U)...
+    intros x x_fresh.
+    rewrite_env (empty ++ [(x, bind_typ S)] ++ E).
+    eapply typing_narrowing_typ_aux...
+    admit.
+Admitted.
+*)
+(*
+Lemma typing_arrow_inversion : forall E f C T1 T2,
+  typing E f (typ_capt C (typ_arrow T1 T2)) ->
+  exists U e L,
+    True. *)
+
+Inductive red (L : atoms) : state -> state -> Prop :=
+  | red_lift : forall x v (v_value : value v) k (k_scope : scope k) S K,
+      x `notin` L ->
+      red L ⟨ S | cont k k_scope :: K | v ⟩
+            ⟨ [(x, store v v_value)] ++ S | K | open_ve k x (`cset_fvar` x) ⟩
+  | red_let_var : forall (x y : atom) v (v_value : value v) k (k_scope : scope k) S K,
+      stores S x v v_value ->
+      red L ⟨ S | cont k k_scope :: K | x ⟩
+            ⟨ S | K | open_ve k x (`cset_fvar` x) ⟩
+  | red_let_val : forall x v (v_value : value v) k (k_scope : scope k) S K,
+      x `notin` L ->
+      red L ⟨ S | K | exp_let v k ⟩
+            ⟨ [(x, store v v_value)] ++ S | K | open_ve k x (`cset_fvar` x) ⟩
+  | red_let_exp : forall e k (k_scope : scope k) S K,
+      red L ⟨ S | K | exp_let e k ⟩
+            ⟨ S | cont k k_scope :: K | e ⟩
+  | red_app : forall f x U e v (v_value : value v) (abs_value : value (exp_abs U e)) S K,
+      stores S f (exp_abs U e) abs_value ->
+      stores S x v v_value ->
+      red L ⟨ S | K | exp_app f x ⟩
+            ⟨ S | K | open_ve e x (`cset_fvar` x) ⟩
+  | red_tapp : forall x T U e (tabs_value : value (exp_tabs U e)) S K,
+      stores S x (exp_tabs U e) tabs_value ->
+      type T ->
+      red L ⟨ S | K | exp_tapp x T ⟩
+            ⟨ S | K | open_te e T ⟩.
+
+Tactic Notation "destructs" constr(E) :=
+  destruct ltac:(applys E).
+Tactic Notation "destructs" constr(E) "as" simple_intropattern(P) :=
+  destruct ltac:(applys E) as P.
+Tactic Notation "destructs" constr(E0) constr(A1) :=
+  destructs (>> E0 A1).
+Tactic Notation "destructs" constr(E0) constr(A1) "as" simple_intropattern(P) :=
+  destructs (>> E0 A1) as P.
+Tactic Notation "destructs" constr(E0) constr(A1) constr(A2) :=
+  destructs (>> E0 A1 A2).
+Tactic Notation "destructs" constr(E0) constr(A1) constr(A2) "as" simple_intropattern(P) :=
+  destructs (>> E0 A1 A2) as P.
+Tactic Notation "destructs" constr(E0) constr(A1) constr(A2) constr(A3) :=
+  destructs (>> E0 A1 A2 A3).
+Tactic Notation "destructs" constr(E0) constr(A1) constr(A2) constr(A3) "as" simple_intropattern(P) :=
+  destructs (>> E0 A1 A2 A3) as P.
+
+Lemma binds_sub_arrow_implies_store_abs' : forall S E C P T1 T2 f,
+  store_typing S E ->
+  binds f (bind_typ (typ_capt C P)) E ->
+  f `~in`A (fv_ct T1 `u`A fv_ct T2) ->
+  sub_pre E P (typ_arrow T1 T2) ->
+  exists U e (abs_value : value (exp_abs U e)), stores S f (exp_abs U e) abs_value /\ sub E T1 U.
+Proof with eauto*.
+  intros * StoreTyp fBinds NotIn Sub.
+  induction StoreTyp; inversion fBinds; subst.
+  destruct (f == x).
+  - inversion H2; subst; clear H2.
+    unfold stores.
+    unfold binds.
+    simpl.
+    destruct (x == x); [ clear e | contradict n; reflexivity ].
+    inversion v_value; subst.
+    + inversion H; subst.
+      * exists T, e1, v_value.
+        inversion Sub; subst.
+        split...
+      * exists T, e1, v_value.
+        split...
+        rewrite_env (empty ++ [(x, bind_typ (typ_capt C P))] ++ E).
+        apply sub_weakening.
+        -- assert (Typ : typing E (exp_abs T e1) (typ_capt C (typ_arrow T1 T2))).
+           { apply typing_sub with (S := typ_capt C P)...
+             rewrite_env (empty ++ [(x, bind_typ (typ_capt C P))] ++ E) in Sub.
+             apply sub_pre_strengthening in Sub.
+             - apply sub_capt...
+               apply subcapt_reflexivity with (A := dom E)...
+             - simpl.
+               repeat apply notin_union...
+               destruct (sub_regular _ _ _ H3) as [_ [_ WfTyp]].
+               eapply wf_pretyp_in_notin_fv_cpt...
+           }
+           applys typing_abs_typ_arrow_implies_sub_param Typ.
+        -- apply wf_env_typ...
+    + assert (Typ : typing E (exp_tabs T e1) (typ_capt C (typ_arrow T1 T2))).
+      { apply typing_sub with (S := typ_capt C P)...
+        rewrite_env (empty ++ [(x, bind_typ (typ_capt C P))] ++ E) in Sub.
+        apply sub_pre_strengthening in Sub.
+        - apply sub_capt...
+          apply subcapt_reflexivity with (A := dom E)...
+        - destruct (sub_pre_regular _ _ _ Sub) as [WfEnv [WfTFun WfS]].
+          simpl.
+          repeat apply notin_union...
+          inversion WfEnv; inversion H6; subst.
+          eapply wf_pretyp_in_notin_fv_cpt...
+      }
+      exfalso.
+      destructs typing_regular Typ as [WfEnv [_ WfArr]].
+      clear - WfEnv WfArr Typ.
+      eremember (exp_tabs T e1) as abs.
+      eremember (typ_capt C (typ_arrow T1 T2)) as arr.
+      assert (Sub : sub E arr (typ_capt C (typ_arrow T1 T2))) by (subst; apply sub_reflexivity with (Ap := dom E) (Am := dom E); eauto* ).
+      clear Heqarr.
+      induction Typ; inversion Heqabs; subst.
+      inversion Sub; inversion H9.
+      apply IHTyp...
+      apply sub_transitivity with (Q := T0)...
+  - assert (Sub' : sub_pre E P (typ_arrow T1 T2)).
+    { rewrite_env (empty ++ [(x, bind_typ T)] ++ E) in Sub.
+      apply sub_pre_strengthening in Sub.
+      - apply Sub.
+      - repeat apply notin_union.
+        + fsetdec.
+        + apply wf_pretyp_in_notin_fv_cpt with (E := E)...
+          enough (WfCP : wf_typ_in E (typ_capt C P)) by (inversion WfCP; eauto* ).
+          apply wf_env_bound_implies_wf_typ with (x := f)...
+        + fold fv_ct.
+          admit.
+        + fold fv_ct.
+          admit.
+    }
+    destruct IHStoreTyp as [U [e [abs_value [xv_S_stores_f T1_sub_U]]]]...
+    exists U, e, abs_value.
+    split.
+    + rewrite_env ([(x, store v v_value)] ++ S).
+      apply binds_tail.
+      * trivial.
+      * simpl; fsetdec.
+    + rewrite_env (empty ++ [(x, bind_typ T)] ++ E).
+      apply sub_weakening...
+Admitted.
+
+Lemma subst_vv_open_vv : forall x u k y v,
+  y <> x ->
+  subst_vv x u (open_vv k y v) = open_vv k y (subst_vv x u v).
+Proof with eauto*.
+  intros * Neq.
+  destruct v; simpl.
+  - destruct (a == x); simpl...
+  - destruct (k === n); simpl...
+    destruct (y == x); simpl; subst...
+Qed.
+
+Lemma subst_ve_open_ve_rec : forall e x y u c1 c2 k,
+  y <> x ->
+  capt c1 ->
+  subst_ve x u c1 (open_ve_rec k y c2 e) =
+    open_ve_rec k y (subst_cset x c1 c2) (subst_ve x u c1 e).
+Proof with auto using subst_vv_open_vv, subst_ct_open_ct_rec.
+  intros * Neq Capt.
+  revert k.
+  induction e; intros k; simpl; f_equal...
+  Check subst_cset_open_cset_rec.
+  Check subst_ct_open_ct_rec.
+  admit.
+  admit.
+  admit.
+Admitted.
+
+(*
+Lemma subcapt_through_subst_ct : forall E S1 C1 C2 x y,
+  wf_env E ->
+  y `~in`A dom E ->
+  binds x (bind_typ S1) E ->
+  subcapt E (open_cset 0 (`cset_fvar` x) C1) C2 ->
+  subcapt ([(y, bind_typ S1)] ++ E) (open_cset 0 (`cset_fvar` y) C1) C2.
+Proof with eauto*.
+  intros * WfEnv NotIn Binds Subcapt.
+  dependent induction Subcapt.
+  - Case "subcapt_universal".
+    apply subcapt_universal.
+    + rewrite_env (empty ++ [(y, bind_typ S1)] ++ E).
+      apply wf_cset_in_weakening...
+      apply ok_cons...
+    + inversion H0; subst.
+      unfold open_cset in H1 |- *.
+      dependent induction C1; simpl in *; simpl_env.
+      destruct_set_mem 0 t0.
+      * rewrite cset_concrete_union in H1 |- *.
+        inversion H1; subst.
+        assert (t0 `c`N {0}N).
+        { clear - OIn H6.
+          intros k kIn.
+          destruct (k === 0); subst.
+          - clear; fsetdec.
+          - assert (k `in`N ({}N `u`N t0 `\`N 0)).
+            { apply NatSet.F.union_3.
+              apply NatSet.F.remove_2...
+            }
+            rewrite <- H6 in H.
+            exfalso.
+            clear - H.
+            destruct (NatSetProperties.Dec.F.empty_iff k)...
+        }
+        clear H6.
+        econstructor.
+        -- intros z zIn.
+           destructs AtomSet.F.union_1 zIn.
+           ++ assert (z = y) by (clear - H4; fsetdec); subst...
+           ++ destruct (H2 z ltac:(fsetdec)) as [T [Bound | Bound]].
+              ** exists T.
+                 apply bound_typ, binds_tail...
+                 simpl.
+                 fsetdec.
+              ** exists T.
+                 apply bound_sub, binds_tail...
+                 simpl.
+                 fsetdec.
+        -- simpl.
+           fsetdec.
+      * rewrite <- H1.
+        rewrite_env (empty ++ [(y, bind_typ S1)] ++ E).
+        apply wf_cset_in_weakening...
+        apply ok_cons...
+  - Case "subcapt_in".
+    inversion H0; subst.
+    unfold open_cset in x |- *.
+    dependent induction C1; simpl in *; simpl_env.
+    destruct_set_mem 0 t0.
+    * rewrite cset_concrete_union in x |- *.
+      inversion x; subst.
+      simpl in x |- *; simpl_env.
+      assert (t0 `c`N {0}N).
+      { clear - OIn H4.
+        intros k kIn.
+        destruct (k === 0); subst.
+        - clear; fsetdec.
+        - assert (k `in`N ({}N `u`N t0 `\`N 0)).
+          { apply NatSet.F.union_3.
+            apply NatSet.F.remove_2...
+          }
+          rewrite <- H4 in H.
+          exfalso.
+          clear - H.
+          destruct (NatSetProperties.Dec.F.empty_iff k)...
+      }
+      clear H4.
+      constructor...
+      -- rewrite_env (empty ++ [(y, bind_typ S1)] ++ E).
+         apply wf_cset_in_weakening...
+         apply ok_cons...
+      -- intros z zIn.
+         destruct (AtomSetProperties.Dec.)
+         eapply subcapt_var. 
+
+
+
+Lemma sub_through_subst_ct : forall E S1 T2 x y U,
+  y `~in`A dom E ->
+  binds x (bind_typ S1) E ->
+  sub E (open_ct T2 (`cset_fvar` x)) U ->
+  sub ([(y, bind_typ S1)] ++ E) (open_ct T2 (`cset_fvar` y)) U
+with sub_pre_through_subst_cpt : forall E S1 P2 x y Q,
+  y `~in`A dom E ->
+  binds x (bind_typ S1) E ->
+  sub_pre E (open_cpt P2 (`cset_fvar` x)) Q ->
+  sub_pre ([(y, bind_typ S1)] ++ E) (open_cpt P2 (`cset_fvar` y)) Q.
+Proof with eauto*.
+{ intros * NotIn Binds Sub.
+  assert (WfEnv : wf_env E) by applys sub_regular Sub.
+  dependent induction Sub.
+  - Case "sub_refl_tvar".
+    unfold open_ct in x |- *.
+    induction T2; simpl in x |- *; simpl_env; subst...
+    inversion x; subst.
+    apply sub_refl_tvar.
+    + apply wf_env_typ...
+      apply wf_env_bound_implies_wf_typ with (x := x0)...
+    + rewrite_env (empty ++ [(y, bind_typ S1)] ++ E).
+      apply wf_typ_in_weakening...
+      apply ok_cons...
+  - Case "sub_trans_tvar".
+    unfold open_ct in x |- *.
+    induction T2; simpl in x |- *; simpl_env; subst...
+    inversion x; subst.
+    eapply sub_trans_tvar with (U := U).
+    + apply binds_tail...
+      simpl.
+      enough (a `in`A dom E) by fsetdec.
+      apply binds_In with (a := bind_sub U), H.
+    + rewrite_env (empty ++ [(y, bind_typ S1)] ++ E).
+      apply sub_weakening...
+      apply wf_env_typ...
+      apply wf_env_bound_implies_wf_typ with (x := x0)...
+  - Case "sub_capt".
+    unfold open_ct in x |- *.
+    induction T2; simpl in x |- *; simpl_env; subst...
+    inversion x; subst.
+    apply sub_capt.
+    + apply wf_env_typ...
+      apply wf_env_bound_implies_wf_typ with (x := x0)...
+    + rewrite_env (empty ++ [(y, bind_typ S1)] ++ E).
+      apply wf_typ_in_weakening...
+      apply ok_cons... 
+
+Lemma eval_typing_through_subst_ct : forall E K S1 T2 U x y,
+  y `~in`A dom E ->
+  binds x (bind_typ S1) E ->
+  eval_typing E K (open_ct T2 (`cset_fvar` x)) U ->
+  eval_typing ([(y, bind_typ S1)] ++ E) K (open_ct T2 (`cset_fvar` y)) U.
+Proof with eauto*.
+  intros * NotIn Binds EvalTyp.
+  assert (WfEnv : wf_env E) by applys eval_typing_regular EvalTyp.
+  dependent induction EvalTyp.
+  - Case "typing_eval_nil".
+    apply typing_eval_nil.
+    + apply wf_env_typ...
+      apply wf_env_bound_implies_wf_typ with (x := x)...
+    + rewrite_env ([(y, bind_typ S1)] ++ E).
+*)
+(*
+Lemma typing_through_subst_ve : forall U E F x T e u C,
+  typing (F ++ [(x, bind_typ U)] ++ E) e T ->
+  x `~in`A fv_cctx F ->
+  binds u (bind_typ U) E ->
+  typing (F ++ E) (subst_ve x u C e) T.
+Proof with simpl_env;
+           eauto 4 using wf_typ_strengthen,
+                         wf_env_strengthening,
+                         sub_strengthening.
+  intros * Typ NotIn uBinds.
+  eremember (F ++ [(x, bind_typ U)] ++ E) as E'.
+  generalize dependent F.
+  induction Typ; intros F EQ NotIn; subst; simpl subst_ve.
+  - Case "typing_var_tvar".
+    destruct (x0 == x); subst.
+    + SCase "x0 = x".
+      binds_get H0.
+      inversion H2; subst.
+      rewrite_env (empty ++ F ++ E).
+      apply typing_weakening...
+      apply wf_env_strengthening_typ in H...
+    + SCase "x0 <> x".
+      binds_cases H0.
+      eauto using wf_env_strengthening_typ.
+      eauto using wf_env_strengthening_typ.
+    - Case "typing_var".
+      destruct (x0 == x); subst.
+      + SCase "x0 = x".
+        binds_get H0.
+        inversion H2; subst; clear H2.
+        rewrite_env (empty ++ F ++ E).
+        apply typing_weakening...
+        apply wf_env_strengthening_typ in H...
+        admit.
+        admit.
+      + SCase "x0 <> x".
+        binds_cases H0.
+        admit.
+        admit.
+  - Case "typing_abs".
+    pick fresh y and apply typing_abs.
+    unfold open_ve.
+    rewrite subst_ve_open_ve_var...
+    rewrite <- concat_assoc.
+
+    (** Now we can apply the induction hypothesis. *)
+
+    apply H0...
+
+  (** The remaining cases in this proof are straightforward, given
+      everything that we have pointed out above. *)
+
+  Case "typing_app".
+    rewrite (if_hoist (f == x) u f var_f).
+    rewrite (if_hoist (x0 == x) u x0 var_f).
+    apply typing_app with (T1 := T1).
+    SCase "callee".
+      rewrite <- (if_hoist (f == x) u f var_f).
+      apply IHTypT1...
+    SCase "argument".
+      rewrite <- (if_hoist (x0 == x) u x0 var_f).
+      apply IHTypT2...
+
+  Case "typing_tabs".
+    pick fresh Y and apply typing_tabs.
+    rewrite subst_ve_open_te_var...
+    rewrite <- concat_assoc.
+    apply H0...
+
+  Case "typing_tapp".
+    rewrite (if_hoist (x0 == x) u x0 var_f).
+    apply typing_tapp with (T1 := T1).
+    SCase "callee".
+      rewrite <- (if_hoist (x0 == x) u x0 var_f).
+      apply IHTypT...
+    SCase "type argument".
+      eauto using sub_strengthening.
+
+  Case "typing_let".
+    pick fresh y and apply typing_let...
+    unfold open_ve.
+    rewrite subst_ve_open_ve_var...
+    rewrite <- concat_assoc.
+    apply H0...
+
+  Case "typing_pair".
+    rewrite (if_hoist (x1 == x) u x1 var_f).
+    rewrite (if_hoist (x2 == x) u x2 var_f).
+    apply typing_pair.
+    SCase "first element".
+      rewrite <- (if_hoist (x1 == x) u x1 var_f).
+      apply IHTypT1...
+    SCase "second element".
+      rewrite <- (if_hoist (x2 == x) u x2 var_f).
+      apply IHTypT2...
+
+  Case "typing_fst".
+    rewrite (if_hoist (x0 == x) u x0 var_f).
+    apply typing_fst with (T2 := T2).
+    rewrite <- (if_hoist (x0 == x) u x0 var_f).
+    apply IHTypT...
+
+  Case "typing_snd".
+    rewrite (if_hoist (x0 == x) u x0 var_f).
+    apply typing_snd with (T1 := T1).
+    rewrite <- (if_hoist (x0 == x) u x0 var_f).
+    apply IHTypT...
+Qed.
+*)
+
+Lemma eval_typing_open : forall E K T U V x y,
+  eval_typing E K (open_ct T (`cset_fvar` x)) U ->
+  eval_typing ([(y, bind_typ V)] ++ E) K (open_ct T (`cset_fvar` y)) U.
+Proof with eauto*.
+  intros * EvalTyp.
+  inversion EvalTyp; subst.
+  admit.
+  admit.
+Admitted.
+
+Lemma preservation : forall s s' V,
+  state_typing s V ->
+  (forall L, red L s s') ->
+  state_typing s' V.
 Ltac hint :=
-    eauto using typing_ctx_sub, wf_cset_set_weakening, wf_sig_weaken_head.
+    eauto using wf_cset_set_weakening.
 Proof with hint.
-  intros * TypState Step.
+  intros * [S K e E T U StoreTyp EvalTyp Typ] Red.
+  induction Typ.
+  - Case "typing_var".
+    inversion EvalTyp; subst.
+    + SCase "typing_eval_nil".
+      specialize (Red {}A); inversion Red; subst; inversion v_value.
+    + SCase "typing_eval_cons".
+      specialize (Red (dom E `u`A L)); inversion Red; subst.
+      * SSCase "red_lift".
+        inversion v_value.
+      * SSCase "red_let_var".
+        apply typing_state with (E := E) (T := U0)...
+        -- apply typing_store_cons...
+           eapply stores_preserves_typing...
+        -- rewrite_env (empty ++ [(y, bind_typ X)] ++ E).
+           apply eval_typing_weakening...
+           apply wf_env_typ...
+           destruct (typing_regular _ _ _ (H1 y (ltac:(fsetdec)))) as [wf_xT_Γ _].
+           inversion wf_xT_Γ; subst...
+  - Case "typing_capt".
+    inversion EvalTyp; subst.
+    + SCase "typing_eval_nil".
+      specialize (Red {}A); inversion Red; subst; inversion v_value.
+    + SCase "typing_eval_cons".
+      specialize (Red (dom E `u`A L)); inversion Red; subst.
+      * SSCase "red_lift".
+        inversion v_value.
+      * SSCase "red_let_var".
+        destructs wf_capt_from_typing_var H H0 as [WfC WfP]...
+        apply typing_state with (E := [(y, bind_typ (typ_capt (`cset_fvar` x) P))] ++ E) (T := U0).
+        -- apply typing_store_cons...
+           eapply stores_preserves_typing...
+        -- rewrite_env (empty ++ [(y, bind_typ (typ_capt (`cset_fvar` x) P))] ++ E).
+           apply eval_typing_weakening...
+           apply wf_env_typ...
+           constructor...
+           constructor...
+           ++ intros z zIn; assert (z = x) by (clear - zIn; fsetdec); subst; clear zIn...
+           ++ enough (x `in`A dom E) by fsetdec.
+              apply binds_In with (a := bind_typ (typ_capt C P))... 
+        -- rewrite_env (empty ++ [(y, bind_typ (typ_capt (`cset_fvar` x) P))] ++ E).
+           specialize (H1 y ltac:(fsetdec)).
+           apply H1.
+  - Case "typing_abs".
+    inversion EvalTyp; subst.
+    + SCase "typing_eval_nil".
+      specialize (Red {}A); inversion Red.
+    + SCase "typing_eval_cons".
+      specialize (Red (dom E `union` L0)); inversion Red; subst.
+      specialize (H3 x ltac:(clear - H11; fsetdec)).
+      apply typing_state with (E := [(x, bind_typ (typ_capt (free_for_cv e1) (typ_arrow V0 T1)))] ++ E) (T := U0); simpl.
+      * SSCase "store_typing".
+        apply typing_store_cons.
+        -- assumption.
+        -- eapply typing_abs...
+        -- clear - H11; fsetdec.
+      * SSCase "eval_typing".
+        rewrite_env (empty ++ [(x, bind_typ (typ_capt (free_for_cv e1) (typ_arrow V0 T1)))] ++ E).
+        apply eval_typing_weakening...
+        applys typing_regular H3.
+      * SSCase "typing".
+        apply H3.
+  - Case "typing_app".
+    clear IHTyp1 IHTyp2.
+    destructs typing_var_inversion Typ1 as [[C [P [fBinds fPSubArr]]] | [X [fBiEnds XSubArr]]].
+    + assert (PSubT1T2 : sub_pre E P (typ_arrow T1 T2)) by (inversion fPSubArr; subst; eauto* ).
+      (* REVIEW: I don't think the following holds but:
+         We have `Γ ⊢ f : C (∀ (x : T1) → T2 x)`
+         If `f ∈ (fv_ct T1 ∪ fv_ct T2)`, we could possibly remove `f` from the
+         capture sets of `T1` and `T2` and lift the dependency on `f` by
+         `Γ ⊢ C <: C ∪ {f}` so that `Γ ⊢ f : (C ∪ {f}) (∀ (x : T1) → T2' x)`
+         where `T1'` and `T2'` are `T1` and `T2` where the dependency on `f`
+         has been removed.
+      *)
+      assert (NotIn : f `~in`A (fv_ct T1 `u`A fv_ct T2)).
+      { admit. }
+      destruct (binds_sub_arrow_implies_store_abs' _ _ _ _ _ _ _ StoreTyp fBinds NotIn PSubT1T2) as [S1 [e [abs_value [fStores T1SubS1]]]].
+      assert (AbsTyp : typing E (exp_abs S1 e) (typ_capt Cf (typ_arrow T1 T2))) by applys stores_preserves_typing StoreTyp fStores Typ1.
+      destruct (typing_inv_abs _ _ _ _ AbsTyp T1 T2 Cf) as [P1 [S2 [L' P2]]].
+      eapply sub_reflexivity with (Ap := dom E) (Am := dom E)...
+      1,2: clear; fsetdec.
+      specialize (Red (dom E `u`A L')); inversion Red; subst.
+      * SCase "red_lift".
+        inversion v_value.
+      * SCase "red_app".
+        eapply typing_state with (E := E) (T := open_ct T2 (`cset_fvar` x))...
+        destruct (P2 y)...
+           
+        apply typing_sub with (S := open_ct S2 (`cset_fvar` x)). 
+        Search (typing _ (open_ve _ _ _) (open_ct _ _)).
+    inversion EvalTyp; subst.
+    + SCase "typing_eval_nil".
+      specialize (Red {}A); inversion Red; subst.
+    + SCase "typing_eval_cons".
+      admit.
+
+
+    destruct (typing_of_var_comes_from_binds _ _ _ Typ1) as [TFun [fBinds SsubT]].
+    destruct (binds_sub_arrow_implies_store_abs _ _ _ _ _ _ _ StoreTyp fBinds SsubT) as [U' [e [abs_value [S_stores_abs T1_sub_U]]]].
+    assert (abs_typing : typing E (exp_abs U' e) (typ_capt Cf (typ_arrow T1 T2))).
+    { apply stores_preserves_typing with (S := S) (E := E) (x := f) (v_value := abs_value)... }
+    destruct (typing_inv_abs _ _ _ _ abs_typing T1 T2 Cf) as [P1 [S2 [L' P2]]].
+    eapply sub_reflexivity...
+    1,2: clear; fsetdec.
+    inversion EvalTyp; subst.
+    + SCase "final".
+      specialize (Red (dom E `u`A L' `u`A fv_ct S2 `u`A (`cset_fvars` (cv U')) `u`A fv_ve (open_ve e x (cv U')))); inversion Red; subst.
+      assert (arg_typing : typing E v T1).
+      { eapply stores_preserves_typing with (x := x) (v_value := v_value)... }
+      assert (exp_abs U' e = exp_abs U0 e0) by applys stores_unique S_stores_abs H7.
+      inversion H2; subst.
+      clear H2.
+      eapply typing_state with (E := E) (T := open_ct T2 (cv T1')); simpl.
+      * SSCase "store_typing".
+        assumption.
+      * SSCase "eval_typing".
+        apply typing_eval_nil...
+      * SSCase "typing".
+        destruct (P2 x) as [xU_E_e_S2 [WfS2 S2subV]]...
+        rewrite_env (empty ++ E).
+        apply typing_sub with (S := open_ct S2 (cv U0))...
+        -- apply typing_strengthening with (x := x) (U := U0).
+           ++ clear - H9; repeat apply notin_union...
+              apply notin_open_ct_rec_fv_ct with (c := cv U0).
+              fsetdec.
+           ++ admit.
+        -- admit.   
+    + SCase "cont".
+      specialize (Red (dom E `u`A L `u`A L' `u`A fv_ve (open_ve e x Cf))); inversion Red; subst.
+      * SSCase "red_lift".
+        inversion v_value.
+      * SSCase "red_app".
+        assert (arg_typing : typing E v T1).
+        { eapply stores_preserves_typing with (x := x) (v_value := v_value)... }
+        eapply typing_state with (E := E) (T := open_ct T2 (cv T1')); simpl...
+        assert (exp_abs U' e = exp_abs U1 e0) by applys stores_unique S_stores_abs H7.
+        inversion H2; subst.
+        clear H2.
+        destruct (P2 x ltac:(fsetdec)).
+        rewrite_env (empty ++ E).
+        apply typing_sub with (S := open_ct S2 (cv T1')).
+        -- apply typing_strengthening with (x := x) (U := U1).
+           ++ clear - H9; repeat apply notin_union...
+              all: admit.
+           ++ admit.
+        -- admit.
+  - Case "typing_let".
+    specialize (Red (dom E `union` L)); inversion Red; subst.
+    * SSCase "red_lift".
+      inversion v_value.
+    * SSCase "red_let_var".
+      eapply typing_state with (E := [(x, bind_typ T1)] ++ E) (T := T2); simpl.
+      -- apply typing_store_cons...
+      -- rewrite_env (empty ++ [(x, bind_typ T1)] ++ E).
+         assert (WfEnv : wf_env ([(x, bind_typ T1)] ++ E)) by applys typing_regular (H x ltac:(fsetdec)).
+         inversion WfEnv; subst.
+         apply eval_typing_weakening...
+      -- apply H...
+    * SSCase "red_let_exp".
+      eapply typing_state with (E := E) (T := T1); simpl.
+      -- assumption.
+      -- apply typing_eval_cons with (L := L) (U := T2)...
+      -- assumption.
+  - Case "typing_tabs".
+    inversion EvalTyp; subst.
+    + SCase "typing_eval_nil".
+      specialize (Red {}A); inversion Red.
+    + SCase "typing_eval_cons".
+      specialize (Red (dom E `union` L0)); inversion Red; subst.
+      specialize (H3 x ltac:(clear - H11; fsetdec)).
+      apply typing_state with (E := [(x, bind_typ (typ_capt (free_for_cv e1) (typ_all V0 T1)))] ++ E) (T := U0); simpl.
+      * SSCase "store_typing".
+        apply typing_store_cons.
+        -- assumption.
+        -- eapply typing_tabs...
+        -- clear - H11; fsetdec.
+      * SSCase "eval_typing".
+        rewrite_env (empty ++ [(x, bind_typ (typ_capt (free_for_cv e1) (typ_all V0 T1)))] ++ E).
+        apply eval_typing_weakening...
+        applys typing_regular H3.
+      * SSCase "typing".
+        apply H3.
+  - Case "typing_tapp".
+    admit.
+  - Case "typing_sub".
+    apply IHTyp...
+    apply eval_typing_contravariant.
+Admitted.   
+
   inversion Step; subst; inversion TypState; subst.
   all: try rename select (typing _ _ _ T) into Typ.
   all: try rename select (typing _ _ _ T0) into Typ.
